Regenerate the test files and add the fstar-split tests

tests/coq/array/Array.v
@@ -12,108 +12,98 @@ Module Array.
     Source: 'src/array.rs', lines 3:0-3:11 *)
 Inductive AB_t := | AB_A : AB_t | AB_B : AB_t.
 
-(** [array::incr]: merged forward/backward function
-    (there is a single backward function, and the forward function returns ())
+(** [array::incr]:
     Source: 'src/array.rs', lines 8:0-8:24 *)
 Definition incr (x : u32) : result u32 :=
   u32_add x 1%u32.
 
-(** [array::array_to_shared_slice_]: forward function
+(** [array::array_to_shared_slice_]:
     Source: 'src/array.rs', lines 16:0-16:53 *)
 Definition array_to_shared_slice_
   (T : Type) (s : array T 32%usize) : result (slice T) :=
   array_to_slice T 32%usize s
 .
 
-(** [array::array_to_mut_slice_]: forward function
+(** [array::array_to_mut_slice_]:
     Source: 'src/array.rs', lines 21:0-21:58 *)
 Definition array_to_mut_slice_
-  (T : Type) (s : array T 32%usize) : result (slice T) :=
-  array_to_slice T 32%usize s
-.
-
-(** [array::array_to_mut_slice_]: backward function 0
-    Source: 'src/array.rs', lines 21:0-21:58 *)
-Definition array_to_mut_slice__back
-  (T : Type) (s : array T 32%usize) (ret : slice T) :
-  result (array T 32%usize)
+  (T : Type) (s : array T 32%usize) :
+  result ((slice T) * (slice T -> result (array T 32%usize)))
   :=
-  array_from_slice T 32%usize s ret
+  p <- array_to_slice_mut T 32%usize s;
+  let (s1, to_slice_mut_back) := p in
+  let back := fun (ret : slice T) => to_slice_mut_back ret in
+  Return (s1, back)
 .
 
-(** [array::array_len]: forward function
+(** [array::array_len]:
     Source: 'src/array.rs', lines 25:0-25:40 *)
 Definition array_len (T : Type) (s : array T 32%usize) : result usize :=
-  s0 <- array_to_slice T 32%usize s; let i := slice_len T s0 in Return i
+  s1 <- array_to_slice T 32%usize s; let i := slice_len T s1 in Return i
 .
 
-(** [array::shared_array_len]: forward function
+(** [array::shared_array_len]:
     Source: 'src/array.rs', lines 29:0-29:48 *)
 Definition shared_array_len (T : Type) (s : array T 32%usize) : result usize :=
-  s0 <- array_to_slice T 32%usize s; let i := slice_len T s0 in Return i
+  s1 <- array_to_slice T 32%usize s; let i := slice_len T s1 in Return i
 .
 
-(** [array::shared_slice_len]: forward function
+(** [array::shared_slice_len]:
     Source: 'src/array.rs', lines 33:0-33:44 *)
 Definition shared_slice_len (T : Type) (s : slice T) : result usize :=
   let i := slice_len T s in Return i
 .
 
-(** [array::index_array_shared]: forward function
+(** [array::index_array_shared]:
     Source: 'src/array.rs', lines 37:0-37:57 *)
 Definition index_array_shared
   (T : Type) (s : array T 32%usize) (i : usize) : result T :=
   array_index_usize T 32%usize s i
 .
 
-(** [array::index_array_u32]: forward function
+(** [array::index_array_u32]:
     Source: 'src/array.rs', lines 44:0-44:53 *)
 Definition index_array_u32 (s : array u32 32%usize) (i : usize) : result u32 :=
   array_index_usize u32 32%usize s i
 .
 
-(** [array::index_array_copy]: forward function
+(** [array::index_array_copy]:
     Source: 'src/array.rs', lines 48:0-48:45 *)
 Definition index_array_copy (x : array u32 32%usize) : result u32 :=
   array_index_usize u32 32%usize x 0%usize
 .
 
-(** [array::index_mut_array]: forward function
+(** [array::index_mut_array]:
     Source: 'src/array.rs', lines 52:0-52:62 *)
 Definition index_mut_array
-  (T : Type) (s : array T 32%usize) (i : usize) : result T :=
-  array_index_usize T 32%usize s i
-.
-
-(** [array::index_mut_array]: backward function 0
-    Source: 'src/array.rs', lines 52:0-52:62 *)
-Definition index_mut_array_back
-  (T : Type) (s : array T 32%usize) (i : usize) (ret : T) :
-  result (array T 32%usize)
+  (T : Type) (s : array T 32%usize) (i : usize) :
+  result (T * (T -> result (array T 32%usize)))
   :=
-  array_update_usize T 32%usize s i ret
+  p <- array_index_mut_usize T 32%usize s i;
+  let (t, index_mut_back) := p in
+  let back := fun (ret : T) => index_mut_back ret in
+  Return (t, back)
 .
 
-(** [array::index_slice]: forward function
+(** [array::index_slice]:
     Source: 'src/array.rs', lines 56:0-56:46 *)
 Definition index_slice (T : Type) (s : slice T) (i : usize) : result T :=
   slice_index_usize T s i
 .
 
-(** [array::index_mut_slice]: forward function
+(** [array::index_mut_slice]:
     Source: 'src/array.rs', lines 60:0-60:58 *)
-Definition index_mut_slice (T : Type) (s : slice T) (i : usize) : result T :=
-  slice_index_usize T s i
+Definition index_mut_slice
+  (T : Type) (s : slice T) (i : usize) :
+  result (T * (T -> result (slice T)))
+  :=
+  p <- slice_index_mut_usize T s i;
+  let (t, index_mut_back) := p in
+  let back := fun (ret : T) => index_mut_back ret in
+  Return (t, back)
 .
 
-(** [array::index_mut_slice]: backward function 0
-    Source: 'src/array.rs', lines 60:0-60:58 *)
-Definition index_mut_slice_back
-  (T : Type) (s : slice T) (i : usize) (ret : T) : result (slice T) :=
-  slice_update_usize T s i ret
-.
-
-(** [array::slice_subslice_shared_]: forward function
+(** [array::slice_subslice_shared_]:
     Source: 'src/array.rs', lines 64:0-64:70 *)
 Definition slice_subslice_shared_
   (x : slice u32) (y : usize) (z : usize) : result (slice u32) :=
@@ -122,47 +112,41 @@ Definition slice_subslice_shared_
     {| core_ops_range_Range_start := y; core_ops_range_Range_end_ := z |}
 .
 
-(** [array::slice_subslice_mut_]: forward function
+(** [array::slice_subslice_mut_]:
     Source: 'src/array.rs', lines 68:0-68:75 *)
 Definition slice_subslice_mut_
-  (x : slice u32) (y : usize) (z : usize) : result (slice u32) :=
-  core_slice_index_Slice_index_mut u32 (core_ops_range_Range usize)
-    (core_slice_index_SliceIndexRangeUsizeSliceTInst u32) x
-    {| core_ops_range_Range_start := y; core_ops_range_Range_end_ := z |}
-.
-
-(** [array::slice_subslice_mut_]: backward function 0
-    Source: 'src/array.rs', lines 68:0-68:75 *)
-Definition slice_subslice_mut__back
-  (x : slice u32) (y : usize) (z : usize) (ret : slice u32) :
-  result (slice u32)
+  (x : slice u32) (y : usize) (z : usize) :
+  result ((slice u32) * (slice u32 -> result (slice u32)))
   :=
-  core_slice_index_Slice_index_mut_back u32 (core_ops_range_Range usize)
-    (core_slice_index_SliceIndexRangeUsizeSliceTInst u32) x
-    {| core_ops_range_Range_start := y; core_ops_range_Range_end_ := z |} ret
+  p <-
+    core_slice_index_Slice_index_mut u32 (core_ops_range_Range usize)
+      (core_slice_index_SliceIndexRangeUsizeSliceTInst u32) x
+      {| core_ops_range_Range_start := y; core_ops_range_Range_end_ := z |};
+  let (s, index_mut_back) := p in
+  let back := fun (ret : slice u32) => index_mut_back ret in
+  Return (s, back)
 .
 
-(** [array::array_to_slice_shared_]: forward function
+(** [array::array_to_slice_shared_]:
     Source: 'src/array.rs', lines 72:0-72:54 *)
 Definition array_to_slice_shared_
   (x : array u32 32%usize) : result (slice u32) :=
   array_to_slice u32 32%usize x
 .
 
-(** [array::array_to_slice_mut_]: forward function
+(** [array::array_to_slice_mut_]:
     Source: 'src/array.rs', lines 76:0-76:59 *)
-Definition array_to_slice_mut_ (x : array u32 32%usize) : result (slice u32) :=
-  array_to_slice u32 32%usize x
+Definition array_to_slice_mut_
+  (x : array u32 32%usize) :
+  result ((slice u32) * (slice u32 -> result (array u32 32%usize)))
+  :=
+  p <- array_to_slice_mut u32 32%usize x;
+  let (s, to_slice_mut_back) := p in
+  let back := fun (ret : slice u32) => to_slice_mut_back ret in
+  Return (s, back)
 .
 
-(** [array::array_to_slice_mut_]: backward function 0
-    Source: 'src/array.rs', lines 76:0-76:59 *)
-Definition array_to_slice_mut__back
-  (x : array u32 32%usize) (ret : slice u32) : result (array u32 32%usize) :=
-  array_from_slice u32 32%usize x ret
-.
-
-(** [array::array_subslice_shared_]: forward function
+(** [array::array_subslice_shared_]:
     Source: 'src/array.rs', lines 80:0-80:74 *)
 Definition array_subslice_shared_
   (x : array u32 32%usize) (y : usize) (z : usize) : result (slice u32) :=
@@ -172,41 +156,35 @@ Definition array_subslice_shared_
     {| core_ops_range_Range_start := y; core_ops_range_Range_end_ := z |}
 .
 
-(** [array::array_subslice_mut_]: forward function
+(** [array::array_subslice_mut_]:
     Source: 'src/array.rs', lines 84:0-84:79 *)
 Definition array_subslice_mut_
-  (x : array u32 32%usize) (y : usize) (z : usize) : result (slice u32) :=
-  core_array_Array_index_mut u32 (core_ops_range_Range usize) 32%usize
-    (core_ops_index_IndexMutSliceTIInst u32 (core_ops_range_Range usize)
-    (core_slice_index_SliceIndexRangeUsizeSliceTInst u32)) x
-    {| core_ops_range_Range_start := y; core_ops_range_Range_end_ := z |}
-.
-
-(** [array::array_subslice_mut_]: backward function 0
-    Source: 'src/array.rs', lines 84:0-84:79 *)
-Definition array_subslice_mut__back
-  (x : array u32 32%usize) (y : usize) (z : usize) (ret : slice u32) :
-  result (array u32 32%usize)
+  (x : array u32 32%usize) (y : usize) (z : usize) :
+  result ((slice u32) * (slice u32 -> result (array u32 32%usize)))
   :=
-  core_array_Array_index_mut_back u32 (core_ops_range_Range usize) 32%usize
-    (core_ops_index_IndexMutSliceTIInst u32 (core_ops_range_Range usize)
-    (core_slice_index_SliceIndexRangeUsizeSliceTInst u32)) x
-    {| core_ops_range_Range_start := y; core_ops_range_Range_end_ := z |} ret
+  p <-
+    core_array_Array_index_mut u32 (core_ops_range_Range usize) 32%usize
+      (core_ops_index_IndexMutSliceTIInst u32 (core_ops_range_Range usize)
+      (core_slice_index_SliceIndexRangeUsizeSliceTInst u32)) x
+      {| core_ops_range_Range_start := y; core_ops_range_Range_end_ := z |};
+  let (s, index_mut_back) := p in
+  let back := fun (ret : slice u32) => index_mut_back ret in
+  Return (s, back)
 .
 
-(** [array::index_slice_0]: forward function
+(** [array::index_slice_0]:
     Source: 'src/array.rs', lines 88:0-88:38 *)
 Definition index_slice_0 (T : Type) (s : slice T) : result T :=
   slice_index_usize T s 0%usize
 .
 
-(** [array::index_array_0]: forward function
+(** [array::index_array_0]:
     Source: 'src/array.rs', lines 92:0-92:42 *)
 Definition index_array_0 (T : Type) (s : array T 32%usize) : result T :=
   array_index_usize T 32%usize s 0%usize
 .
 
-(** [array::index_index_array]: forward function
+(** [array::index_index_array]:
     Source: 'src/array.rs', lines 103:0-103:71 *)
 Definition index_index_array
   (s : array (array u32 32%usize) 32%usize) (i : usize) (j : usize) :
@@ -216,157 +194,164 @@ Definition index_index_array
   array_index_usize u32 32%usize a j
 .
 
-(** [array::update_update_array]: forward function
+(** [array::update_update_array]:
     Source: 'src/array.rs', lines 114:0-114:70 *)
 Definition update_update_array
   (s : array (array u32 32%usize) 32%usize) (i : usize) (j : usize) :
   result unit
   :=
-  a <- array_index_usize (array u32 32%usize) 32%usize s i;
-  a0 <- array_update_usize u32 32%usize a j 0%u32;
-  _ <- array_update_usize (array u32 32%usize) 32%usize s i a0;
+  p <- array_index_mut_usize (array u32 32%usize) 32%usize s i;
+  let (a, index_mut_back) := p in
+  p1 <- array_index_mut_usize u32 32%usize a j;
+  let (_, index_mut_back1) := p1 in
+  a1 <- index_mut_back1 0%u32;
+  _ <- index_mut_back a1;
   Return tt
 .
 
-(** [array::array_local_deep_copy]: forward function
+(** [array::array_local_deep_copy]:
     Source: 'src/array.rs', lines 118:0-118:43 *)
 Definition array_local_deep_copy (x : array u32 32%usize) : result unit :=
   Return tt
 .
 
-(** [array::take_array]: forward function
+(** [array::take_array]:
     Source: 'src/array.rs', lines 122:0-122:30 *)
 Definition take_array (a : array u32 2%usize) : result unit :=
   Return tt.
 
-(** [array::take_array_borrow]: forward function
+(** [array::take_array_borrow]:
     Source: 'src/array.rs', lines 123:0-123:38 *)
 Definition take_array_borrow (a : array u32 2%usize) : result unit :=
   Return tt
 .
 
-(** [array::take_slice]: forward function
+(** [array::take_slice]:
     Source: 'src/array.rs', lines 124:0-124:28 *)
 Definition take_slice (s : slice u32) : result unit :=
   Return tt.
 
-(** [array::take_mut_slice]: merged forward/backward function
-    (there is a single backward function, and the forward function returns ())
+(** [array::take_mut_slice]:
     Source: 'src/array.rs', lines 125:0-125:36 *)
 Definition take_mut_slice (s : slice u32) : result (slice u32) :=
   Return s.
 
-(** [array::const_array]: forward function
+(** [array::const_array]:
     Source: 'src/array.rs', lines 127:0-127:32 *)
 Definition const_array : result (array u32 2%usize) :=
   Return (mk_array u32 2%usize [ 0%u32; 0%u32 ])
 .
 
-(** [array::const_slice]: forward function
+(** [array::const_slice]:
     Source: 'src/array.rs', lines 131:0-131:20 *)
 Definition const_slice : result unit :=
   _ <- array_to_slice u32 2%usize (mk_array u32 2%usize [ 0%u32; 0%u32 ]);
   Return tt
 .
 
-(** [array::take_all]: forward function
+(** [array::take_all]:
     Source: 'src/array.rs', lines 141:0-141:17 *)
 Definition take_all : result unit :=
+  _ <- take_array (mk_array u32 2%usize [ 0%u32; 0%u32 ]);
   _ <- take_array (mk_array u32 2%usize [ 0%u32; 0%u32 ]);
   _ <- take_array_borrow (mk_array u32 2%usize [ 0%u32; 0%u32 ]);
   s <- array_to_slice u32 2%usize (mk_array u32 2%usize [ 0%u32; 0%u32 ]);
   _ <- take_slice s;
-  s0 <- array_to_slice u32 2%usize (mk_array u32 2%usize [ 0%u32; 0%u32 ]);
-  s1 <- take_mut_slice s0;
-  _ <- array_from_slice u32 2%usize (mk_array u32 2%usize [ 0%u32; 0%u32 ]) s1;
+  p <- array_to_slice_mut u32 2%usize (mk_array u32 2%usize [ 0%u32; 0%u32 ]);
+  let (s1, to_slice_mut_back) := p in
+  s2 <- take_mut_slice s1;
+  _ <- to_slice_mut_back s2;
   Return tt
 .
 
-(** [array::index_array]: forward function
+(** [array::index_array]:
     Source: 'src/array.rs', lines 155:0-155:38 *)
 Definition index_array (x : array u32 2%usize) : result u32 :=
   array_index_usize u32 2%usize x 0%usize
 .
 
-(** [array::index_array_borrow]: forward function
+(** [array::index_array_borrow]:
     Source: 'src/array.rs', lines 158:0-158:46 *)
 Definition index_array_borrow (x : array u32 2%usize) : result u32 :=
   array_index_usize u32 2%usize x 0%usize
 .
 
-(** [array::index_slice_u32_0]: forward function
+(** [array::index_slice_u32_0]:
     Source: 'src/array.rs', lines 162:0-162:42 *)
 Definition index_slice_u32_0 (x : slice u32) : result u32 :=
   slice_index_usize u32 x 0%usize
 .
 
-(** [array::index_mut_slice_u32_0]: forward function
+(** [array::index_mut_slice_u32_0]:
     Source: 'src/array.rs', lines 166:0-166:50 *)
-Definition index_mut_slice_u32_0 (x : slice u32) : result u32 :=
-  slice_index_usize u32 x 0%usize
+Definition index_mut_slice_u32_0
+  (x : slice u32) : result (u32 * (slice u32)) :=
+  i <- slice_index_usize u32 x 0%usize; Return (i, x)
 .
 
-(** [array::index_mut_slice_u32_0]: backward function 0
-    Source: 'src/array.rs', lines 166:0-166:50 *)
-Definition index_mut_slice_u32_0_back (x : slice u32) : result (slice u32) :=
-  _ <- slice_index_usize u32 x 0%usize; Return x
-.
-
-(** [array::index_all]: forward function
+(** [array::index_all]:
     Source: 'src/array.rs', lines 170:0-170:25 *)
 Definition index_all : result u32 :=
   i <- index_array (mk_array u32 2%usize [ 0%u32; 0%u32 ]);
-  i0 <- index_array (mk_array u32 2%usize [ 0%u32; 0%u32 ]);
-  i1 <- u32_add i i0;
-  i2 <- index_array_borrow (mk_array u32 2%usize [ 0%u32; 0%u32 ]);
-  i3 <- u32_add i1 i2;
+  i1 <- index_array (mk_array u32 2%usize [ 0%u32; 0%u32 ]);
+  i2 <- u32_add i i1;
+  i3 <- index_array_borrow (mk_array u32 2%usize [ 0%u32; 0%u32 ]);
+  i4 <- u32_add i2 i3;
   s <- array_to_slice u32 2%usize (mk_array u32 2%usize [ 0%u32; 0%u32 ]);
-  i4 <- index_slice_u32_0 s;
-  i5 <- u32_add i3 i4;
-  s0 <- array_to_slice u32 2%usize (mk_array u32 2%usize [ 0%u32; 0%u32 ]);
-  i6 <- index_mut_slice_u32_0 s0;
-  i7 <- u32_add i5 i6;
-  s1 <- index_mut_slice_u32_0_back s0;
-  _ <- array_from_slice u32 2%usize (mk_array u32 2%usize [ 0%u32; 0%u32 ]) s1;
-  Return i7
+  i5 <- index_slice_u32_0 s;
+  i6 <- u32_add i4 i5;
+  p <- array_to_slice_mut u32 2%usize (mk_array u32 2%usize [ 0%u32; 0%u32 ]);
+  let (s1, to_slice_mut_back) := p in
+  p1 <- index_mut_slice_u32_0 s1;
+  let (i7, s2) := p1 in
+  i8 <- u32_add i6 i7;
+  _ <- to_slice_mut_back s2;
+  Return i8
 .
 
-(** [array::update_array]: forward function
+(** [array::update_array]:
     Source: 'src/array.rs', lines 184:0-184:36 *)
 Definition update_array (x : array u32 2%usize) : result unit :=
-  _ <- array_update_usize u32 2%usize x 0%usize 1%u32; Return tt
-.
-
-(** [array::update_array_mut_borrow]: merged forward/backward function
-    (there is a single backward function, and the forward function returns ())
-    Source: 'src/array.rs', lines 187:0-187:48 *)
-Definition update_array_mut_borrow
-  (x : array u32 2%usize) : result (array u32 2%usize) :=
-  array_update_usize u32 2%usize x 0%usize 1%u32
-.
-
-(** [array::update_mut_slice]: merged forward/backward function
-    (there is a single backward function, and the forward function returns ())
-    Source: 'src/array.rs', lines 190:0-190:38 *)
-Definition update_mut_slice (x : slice u32) : result (slice u32) :=
-  slice_update_usize u32 x 0%usize 1%u32
-.
-
-(** [array::update_all]: forward function
-    Source: 'src/array.rs', lines 194:0-194:19 *)
-Definition update_all : result unit :=
-  _ <- update_array (mk_array u32 2%usize [ 0%u32; 0%u32 ]);
-  x <- update_array_mut_borrow (mk_array u32 2%usize [ 0%u32; 0%u32 ]);
-  s <- array_to_slice u32 2%usize x;
-  s0 <- update_mut_slice s;
-  _ <- array_from_slice u32 2%usize x s0;
+  p <- array_index_mut_usize u32 2%usize x 0%usize;
+  let (_, index_mut_back) := p in
+  _ <- index_mut_back 1%u32;
   Return tt
 .
 
-(** [array::range_all]: forward function
+(** [array::update_array_mut_borrow]:
+    Source: 'src/array.rs', lines 187:0-187:48 *)
+Definition update_array_mut_borrow
+  (x : array u32 2%usize) : result (array u32 2%usize) :=
+  p <- array_index_mut_usize u32 2%usize x 0%usize;
+  let (_, index_mut_back) := p in
+  index_mut_back 1%u32
+.
+
+(** [array::update_mut_slice]:
+    Source: 'src/array.rs', lines 190:0-190:38 *)
+Definition update_mut_slice (x : slice u32) : result (slice u32) :=
+  p <- slice_index_mut_usize u32 x 0%usize;
+  let (_, index_mut_back) := p in
+  index_mut_back 1%u32
+.
+
+(** [array::update_all]:
+    Source: 'src/array.rs', lines 194:0-194:19 *)
+Definition update_all : result unit :=
+  _ <- update_array (mk_array u32 2%usize [ 0%u32; 0%u32 ]);
+  _ <- update_array (mk_array u32 2%usize [ 0%u32; 0%u32 ]);
+  a <- update_array_mut_borrow (mk_array u32 2%usize [ 0%u32; 0%u32 ]);
+  p <- array_to_slice_mut u32 2%usize a;
+  let (s, to_slice_mut_back) := p in
+  s1 <- update_mut_slice s;
+  _ <- to_slice_mut_back s1;
+  Return tt
+.
+
+(** [array::range_all]:
     Source: 'src/array.rs', lines 205:0-205:18 *)
 Definition range_all : result unit :=
-  s <-
+  p <-
     core_array_Array_index_mut u32 (core_ops_range_Range usize) 4%usize
       (core_ops_index_IndexMutSliceTIInst u32 (core_ops_range_Range usize)
       (core_slice_index_SliceIndexRangeUsizeSliceTInst u32))
@@ -375,127 +360,119 @@ Definition range_all : result unit :=
         core_ops_range_Range_start := 1%usize;
         core_ops_range_Range_end_ := 3%usize
       |};
-  s0 <- update_mut_slice s;
-  _ <-
-    core_array_Array_index_mut_back u32 (core_ops_range_Range usize) 4%usize
-      (core_ops_index_IndexMutSliceTIInst u32 (core_ops_range_Range usize)
-      (core_slice_index_SliceIndexRangeUsizeSliceTInst u32))
-      (mk_array u32 4%usize [ 0%u32; 0%u32; 0%u32; 0%u32 ])
-      {|
-        core_ops_range_Range_start := 1%usize;
-        core_ops_range_Range_end_ := 3%usize
-      |} s0;
+  let (s, index_mut_back) := p in
+  s1 <- update_mut_slice s;
+  _ <- index_mut_back s1;
   Return tt
 .
 
-(** [array::deref_array_borrow]: forward function
+(** [array::deref_array_borrow]:
     Source: 'src/array.rs', lines 214:0-214:46 *)
 Definition deref_array_borrow (x : array u32 2%usize) : result u32 :=
   array_index_usize u32 2%usize x 0%usize
 .
 
-(** [array::deref_array_mut_borrow]: forward function
+(** [array::deref_array_mut_borrow]:
     Source: 'src/array.rs', lines 219:0-219:54 *)
-Definition deref_array_mut_borrow (x : array u32 2%usize) : result u32 :=
-  array_index_usize u32 2%usize x 0%usize
+Definition deref_array_mut_borrow
+  (x : array u32 2%usize) : result (u32 * (array u32 2%usize)) :=
+  i <- array_index_usize u32 2%usize x 0%usize; Return (i, x)
 .
 
-(** [array::deref_array_mut_borrow]: backward function 0
-    Source: 'src/array.rs', lines 219:0-219:54 *)
-Definition deref_array_mut_borrow_back
-  (x : array u32 2%usize) : result (array u32 2%usize) :=
-  _ <- array_index_usize u32 2%usize x 0%usize; Return x
-.
-
-(** [array::take_array_t]: forward function
+(** [array::take_array_t]:
     Source: 'src/array.rs', lines 227:0-227:31 *)
 Definition take_array_t (a : array AB_t 2%usize) : result unit :=
   Return tt.
 
-(** [array::non_copyable_array]: forward function
+(** [array::non_copyable_array]:
     Source: 'src/array.rs', lines 229:0-229:27 *)
 Definition non_copyable_array : result unit :=
   _ <- take_array_t (mk_array AB_t 2%usize [ AB_A; AB_B ]); Return tt
 .
 
-(** [array::sum]: loop 0: forward function
+(** [array::sum]: loop 0:
     Source: 'src/array.rs', lines 242:0-250:1 *)
 Fixpoint sum_loop
-  (n : nat) (s : slice u32) (sum0 : u32) (i : usize) : result u32 :=
+  (n : nat) (s : slice u32) (sum1 : u32) (i : usize) : result u32 :=
   match n with
   | O => Fail_ OutOfFuel
-  | S n0 =>
-    let i0 := slice_len u32 s in
-    if i s< i0
+  | S n1 =>
+    let i1 := slice_len u32 s in
+    if i s< i1
     then (
-      i1 <- slice_index_usize u32 s i;
-      sum1 <- u32_add sum0 i1;
-      i2 <- usize_add i 1%usize;
-      sum_loop n0 s sum1 i2)
-    else Return sum0
+      i2 <- slice_index_usize u32 s i;
+      sum3 <- u32_add sum1 i2;
+      i3 <- usize_add i 1%usize;
+      sum_loop n1 s sum3 i3)
+    else Return sum1
   end
 .
 
-(** [array::sum]: forward function
+(** [array::sum]:
     Source: 'src/array.rs', lines 242:0-242:28 *)
 Definition sum (n : nat) (s : slice u32) : result u32 :=
   sum_loop n s 0%u32 0%usize
 .
 
-(** [array::sum2]: loop 0: forward function
+(** [array::sum2]: loop 0:
     Source: 'src/array.rs', lines 252:0-261:1 *)
 Fixpoint sum2_loop
-  (n : nat) (s : slice u32) (s2 : slice u32) (sum0 : u32) (i : usize) :
+  (n : nat) (s : slice u32) (s2 : slice u32) (sum1 : u32) (i : usize) :
   result u32
   :=
   match n with
   | O => Fail_ OutOfFuel
-  | S n0 =>
-    let i0 := slice_len u32 s in
-    if i s< i0
+  | S n1 =>
+    let i1 := slice_len u32 s in
+    if i s< i1
     then (
-      i1 <- slice_index_usize u32 s i;
-      i2 <- slice_index_usize u32 s2 i;
-      i3 <- u32_add i1 i2;
-      sum1 <- u32_add sum0 i3;
-      i4 <- usize_add i 1%usize;
-      sum2_loop n0 s s2 sum1 i4)
-    else Return sum0
+      i2 <- slice_index_usize u32 s i;
+      i3 <- slice_index_usize u32 s2 i;
+      i4 <- u32_add i2 i3;
+      sum3 <- u32_add sum1 i4;
+      i5 <- usize_add i 1%usize;
+      sum2_loop n1 s s2 sum3 i5)
+    else Return sum1
   end
 .
 
-(** [array::sum2]: forward function
+(** [array::sum2]:
     Source: 'src/array.rs', lines 252:0-252:41 *)
 Definition sum2 (n : nat) (s : slice u32) (s2 : slice u32) : result u32 :=
   let i := slice_len u32 s in
-  let i0 := slice_len u32 s2 in
-  if negb (i s= i0) then Fail_ Failure else sum2_loop n s s2 0%u32 0%usize
+  let i1 := slice_len u32 s2 in
+  if negb (i s= i1) then Fail_ Failure else sum2_loop n s s2 0%u32 0%usize
 .
 
-(** [array::f0]: forward function
+(** [array::f0]:
     Source: 'src/array.rs', lines 263:0-263:11 *)
 Definition f0 : result unit :=
-  s <- array_to_slice u32 2%usize (mk_array u32 2%usize [ 1%u32; 2%u32 ]);
-  s0 <- slice_update_usize u32 s 0%usize 1%u32;
-  _ <- array_from_slice u32 2%usize (mk_array u32 2%usize [ 1%u32; 2%u32 ]) s0;
+  p <- array_to_slice_mut u32 2%usize (mk_array u32 2%usize [ 1%u32; 2%u32 ]);
+  let (s, to_slice_mut_back) := p in
+  p1 <- slice_index_mut_usize u32 s 0%usize;
+  let (_, index_mut_back) := p1 in
+  s1 <- index_mut_back 1%u32;
+  _ <- to_slice_mut_back s1;
   Return tt
 .
 
-(** [array::f1]: forward function
+(** [array::f1]:
     Source: 'src/array.rs', lines 268:0-268:11 *)
 Definition f1 : result unit :=
-  _ <-
-    array_update_usize u32 2%usize (mk_array u32 2%usize [ 1%u32; 2%u32 ])
-      0%usize 1%u32;
+  p <-
+    array_index_mut_usize u32 2%usize (mk_array u32 2%usize [ 1%u32; 2%u32 ])
+      0%usize;
+  let (_, index_mut_back) := p in
+  _ <- index_mut_back 1%u32;
   Return tt
 .
 
-(** [array::f2]: forward function
+(** [array::f2]:
     Source: 'src/array.rs', lines 273:0-273:17 *)
 Definition f2 (i : u32) : result unit :=
   Return tt.
 
-(** [array::f4]: forward function
+(** [array::f4]:
     Source: 'src/array.rs', lines 282:0-282:54 *)
 Definition f4
   (x : array u32 32%usize) (y : usize) (z : usize) : result (slice u32) :=
@@ -505,7 +482,7 @@ Definition f4
     {| core_ops_range_Range_start := y; core_ops_range_Range_end_ := z |}
 .
 
-(** [array::f3]: forward function
+(** [array::f3]:
     Source: 'src/array.rs', lines 275:0-275:18 *)
 Definition f3 (n : nat) : result u32 :=
   i <-
@@ -514,8 +491,8 @@ Definition f3 (n : nat) : result u32 :=
   _ <- f2 i;
   let b := array_repeat u32 32%usize 0%u32 in
   s <- array_to_slice u32 2%usize (mk_array u32 2%usize [ 1%u32; 2%u32 ]);
-  s0 <- f4 b 16%usize 18%usize;
-  sum2 n s s0
+  s1 <- f4 b 16%usize 18%usize;
+  sum2 n s s1
 .
 
 (** [array::SZ]
@@ -523,21 +500,25 @@ Definition f3 (n : nat) : result u32 :=
 Definition sz_body : result usize := Return 32%usize.
 Definition sz_c : usize := sz_body%global.
 
-(** [array::f5]: forward function
+(** [array::f5]:
     Source: 'src/array.rs', lines 289:0-289:31 *)
 Definition f5 (x : array u32 32%usize) : result u32 :=
   array_index_usize u32 32%usize x 0%usize
 .
 
-(** [array::ite]: forward function
+(** [array::ite]:
     Source: 'src/array.rs', lines 294:0-294:12 *)
 Definition ite : result unit :=
-  s <- array_to_slice u32 2%usize (mk_array u32 2%usize [ 0%u32; 0%u32 ]);
-  s0 <- array_to_slice u32 2%usize (mk_array u32 2%usize [ 0%u32; 0%u32 ]);
-  s1 <- index_mut_slice_u32_0_back s0;
-  _ <- array_from_slice u32 2%usize (mk_array u32 2%usize [ 0%u32; 0%u32 ]) s1;
-  s2 <- index_mut_slice_u32_0_back s;
-  _ <- array_from_slice u32 2%usize (mk_array u32 2%usize [ 0%u32; 0%u32 ]) s2;
+  p <- array_to_slice_mut u32 2%usize (mk_array u32 2%usize [ 0%u32; 0%u32 ]);
+  let (s, to_slice_mut_back) := p in
+  p1 <- index_mut_slice_u32_0 s;
+  let (_, s1) := p1 in
+  p2 <- array_to_slice_mut u32 2%usize (mk_array u32 2%usize [ 0%u32; 0%u32 ]);
+  let (s2, to_slice_mut_back1) := p2 in
+  p3 <- index_mut_slice_u32_0 s2;
+  let (_, s3) := p3 in
+  _ <- to_slice_mut_back1 s3;
+  _ <- to_slice_mut_back s1;
   Return tt
 .
 
