tests/coq/misc/Paper.v
@@ -8,44 +8,40 @@ Import ListNotations.
 Local Open Scope Primitives_scope.
 Module Paper.
 
-(** [paper::ref_incr]: merged forward/backward function
-    (there is a single backward function, and the forward function returns ())
+(** [paper::ref_incr]:
     Source: 'src/paper.rs', lines 4:0-4:28 *)
 Definition ref_incr (x : i32) : result i32 :=
   i32_add x 1%i32.
 
-(** [paper::test_incr]: forward function
+(** [paper::test_incr]:
     Source: 'src/paper.rs', lines 8:0-8:18 *)
 Definition test_incr : result unit :=
-  x <- ref_incr 0%i32; if negb (x s= 1%i32) then Fail_ Failure else Return tt
+  i <- ref_incr 0%i32; if negb (i s= 1%i32) then Fail_ Failure else Return tt
 .
 
 (** Unit test for [paper::test_incr] *)
 Check (test_incr )%return.
 
-(** [paper::choose]: forward function
+(** [paper::choose]:
     Source: 'src/paper.rs', lines 15:0-15:70 *)
-Definition choose (T : Type) (b : bool) (x : T) (y : T) : result T :=
-  if b then Return x else Return y
+Definition choose
+  (T : Type) (b : bool) (x : T) (y : T) : result (T * (T -> result (T * T))) :=
+  if b
+  then let back_'a := fun (ret : T) => Return (ret, y) in Return (x, back_'a)
+  else let back_'a := fun (ret : T) => Return (x, ret) in Return (y, back_'a)
 .
 
-(** [paper::choose]: backward function 0
-    Source: 'src/paper.rs', lines 15:0-15:70 *)
-Definition choose_back
-  (T : Type) (b : bool) (x : T) (y : T) (ret : T) : result (T * T) :=
-  if b then Return (ret, y) else Return (x, ret)
-.
-
-(** [paper::test_choose]: forward function
+(** [paper::test_choose]:
     Source: 'src/paper.rs', lines 23:0-23:20 *)
 Definition test_choose : result unit :=
-  z <- choose i32 true 0%i32 0%i32;
-  z0 <- i32_add z 1%i32;
-  if negb (z0 s= 1%i32)
+  p <- choose i32 true 0%i32 0%i32;
+  let (z, choose_back) := p in
+  z1 <- i32_add z 1%i32;
+  if negb (z1 s= 1%i32)
   then Fail_ Failure
   else (
-    p <- choose_back i32 true 0%i32 0%i32 z0;
-    let (x, y) := p in
+    p1 <- choose_back z1;
+    let (x, y) := p1 in
     if negb (x s= 1%i32)
     then Fail_ Failure
     else if negb (y s= 0%i32) then Fail_ Failure else Return tt)
@@ -64,35 +60,31 @@ Inductive List_t (T : Type) :=
 Arguments List_Cons { _ }.
 Arguments List_Nil { _ }.
 
-(** [paper::list_nth_mut]: forward function
+(** [paper::list_nth_mut]:
     Source: 'src/paper.rs', lines 42:0-42:67 *)
-Fixpoint list_nth_mut (T : Type) (l : List_t T) (i : u32) : result T :=
+Fixpoint list_nth_mut
+  (T : Type) (l : List_t T) (i : u32) :
+  result (T * (T -> result (List_t T)))
+  :=
   match l with
   | List_Cons x tl =>
     if i s= 0%u32
-    then Return x
-    else (i0 <- u32_sub i 1%u32; list_nth_mut T tl i0)
-  | List_Nil => Fail_ Failure
-  end
-.
-
-(** [paper::list_nth_mut]: backward function 0
-    Source: 'src/paper.rs', lines 42:0-42:67 *)
-Fixpoint list_nth_mut_back
-  (T : Type) (l : List_t T) (i : u32) (ret : T) : result (List_t T) :=
-  match l with
-  | List_Cons x tl =>
-    if i s= 0%u32
-    then Return (List_Cons ret tl)
+    then
+      let back_'a := fun (ret : T) => Return (List_Cons ret tl) in
+      Return (x, back_'a)
     else (
-      i0 <- u32_sub i 1%u32;
-      tl0 <- list_nth_mut_back T tl i0 ret;
-      Return (List_Cons x tl0))
+      i1 <- u32_sub i 1%u32;
+      p <- list_nth_mut T tl i1;
+      let (t, list_nth_mut_back) := p in
+      let back_'a :=
+        fun (ret : T) => tl1 <- list_nth_mut_back ret; Return (List_Cons x tl1)
+        in
+      Return (t, back_'a))
   | List_Nil => Fail_ Failure
   end
 .
 
-(** [paper::sum]: forward function
+(** [paper::sum]:
     Source: 'src/paper.rs', lines 57:0-57:32 *)
 Fixpoint sum (l : List_t i32) : result i32 :=
   match l with
@@ -101,31 +93,33 @@ Fixpoint sum (l : List_t i32) : result i32 :=
   end
 .
 
-(** [paper::test_nth]: forward function
+(** [paper::test_nth]:
     Source: 'src/paper.rs', lines 68:0-68:17 *)
 Definition test_nth : result unit :=
   let l := List_Nil in
-  let l0 := List_Cons 3%i32 l in
-  let l1 := List_Cons 2%i32 l0 in
-  x <- list_nth_mut i32 (List_Cons 1%i32 l1) 2%u32;
-  x0 <- i32_add x 1%i32;
-  l2 <- list_nth_mut_back i32 (List_Cons 1%i32 l1) 2%u32 x0;
-  i <- sum l2;
+  let l1 := List_Cons 3%i32 l in
+  let l2 := List_Cons 2%i32 l1 in
+  p <- list_nth_mut i32 (List_Cons 1%i32 l2) 2%u32;
+  let (x, list_nth_mut_back) := p in
+  x1 <- i32_add x 1%i32;
+  l3 <- list_nth_mut_back x1;
+  i <- sum l3;
   if negb (i s= 7%i32) then Fail_ Failure else Return tt
 .
 
 (** Unit test for [paper::test_nth] *)
 Check (test_nth )%return.
 
-(** [paper::call_choose]: forward function
+(** [paper::call_choose]:
     Source: 'src/paper.rs', lines 76:0-76:44 *)
 Definition call_choose (p : (u32 * u32)) : result u32 :=
   let (px, py) := p in
-  pz <- choose u32 true px py;
-  pz0 <- u32_add pz 1%u32;
-  p0 <- choose_back u32 true px py pz0;
-  let (px0, _) := p0 in
-  Return px0
+  p1 <- choose u32 true px py;
+  let (pz, choose_back) := p1 in
+  pz1 <- u32_add pz 1%u32;
+  p2 <- choose_back pz1;
+  let (px1, _) := p2 in
+  Return px1
 .
 
 End Paper.
