tests/fstar/hashmap/Hashmap.Funs.fst
@@ -7,12 +7,12 @@ include Hashmap.Clauses
 
 #set-options "--z3rlimit 50 --fuel 1 --ifuel 1"
 
-(** [hashmap::hash_key]: forward function
+(** [hashmap::hash_key]:
     Source: 'src/hashmap.rs', lines 27:0-27:32 *)
 let hash_key (k : usize) : result usize =
   Return k
 
-(** [hashmap::{hashmap::HashMap<T>}::allocate_slots]: loop 0: forward function
+(** [hashmap::{hashmap::HashMap<T>}::allocate_slots]: loop 0:
     Source: 'src/hashmap.rs', lines 50:4-56:5 *)
 let rec hashMap_allocate_slots_loop
   (t : Type0) (slots : alloc_vec_Vec (list_t t)) (n : usize) :
@@ -21,12 +21,12 @@ let rec hashMap_allocate_slots_loop
   =
   if n > 0
   then
-    let* slots0 = alloc_vec_Vec_push (list_t t) slots List_Nil in
-    let* n0 = usize_sub n 1 in
-    hashMap_allocate_slots_loop t slots0 n0
+    let* v = alloc_vec_Vec_push (list_t t) slots List_Nil in
+    let* n1 = usize_sub n 1 in
+    hashMap_allocate_slots_loop t v n1
   else Return slots
 
-(** [hashmap::{hashmap::HashMap<T>}::allocate_slots]: forward function
+(** [hashmap::{hashmap::HashMap<T>}::allocate_slots]:
     Source: 'src/hashmap.rs', lines 50:4-50:76 *)
 let hashMap_allocate_slots
   (t : Type0) (slots : alloc_vec_Vec (list_t t)) (n : usize) :
@@ -34,7 +34,7 @@ let hashMap_allocate_slots
   =
   hashMap_allocate_slots_loop t slots n
 
-(** [hashmap::{hashmap::HashMap<T>}::new_with_capacity]: forward function
+(** [hashmap::{hashmap::HashMap<T>}::new_with_capacity]:
     Source: 'src/hashmap.rs', lines 59:4-63:13 *)
 let hashMap_new_with_capacity
   (t : Type0) (capacity : usize) (max_load_dividend : usize)
@@ -44,97 +44,75 @@ let hashMap_new_with_capacity
   let v = alloc_vec_Vec_new (list_t t) in
   let* slots = hashMap_allocate_slots t v capacity in
   let* i = usize_mul capacity max_load_dividend in
-  let* i0 = usize_div i max_load_divisor in
+  let* i1 = usize_div i max_load_divisor in
   Return
     {
       num_entries = 0;
       max_load_factor = (max_load_dividend, max_load_divisor);
-      max_load = i0;
+      max_load = i1;
       slots = slots
     }
 
-(** [hashmap::{hashmap::HashMap<T>}::new]: forward function
+(** [hashmap::{hashmap::HashMap<T>}::new]:
     Source: 'src/hashmap.rs', lines 75:4-75:24 *)
 let hashMap_new (t : Type0) : result (hashMap_t t) =
   hashMap_new_with_capacity t 32 4 5
 
-(** [hashmap::{hashmap::HashMap<T>}::clear]: loop 0: merged forward/backward function
-    (there is a single backward function, and the forward function returns ())
+(** [hashmap::{hashmap::HashMap<T>}::clear]: loop 0:
     Source: 'src/hashmap.rs', lines 80:4-88:5 *)
 let rec hashMap_clear_loop
   (t : Type0) (slots : alloc_vec_Vec (list_t t)) (i : usize) :
   Tot (result (alloc_vec_Vec (list_t t)))
   (decreases (hashMap_clear_loop_decreases t slots i))
   =
-  let i0 = alloc_vec_Vec_len (list_t t) slots in
-  if i < i0
+  let i1 = alloc_vec_Vec_len (list_t t) slots in
+  if i < i1
   then
-    let* i1 = usize_add i 1 in
-    let* slots0 =
-      alloc_vec_Vec_index_mut_back (list_t t) usize
-        (core_slice_index_SliceIndexUsizeSliceTInst (list_t t)) slots i
-        List_Nil in
-    hashMap_clear_loop t slots0 i1
+    let* (_, index_mut_back) =
+      alloc_vec_Vec_index_mut (list_t t) usize
+        (core_slice_index_SliceIndexUsizeSliceTInst (list_t t)) slots i in
+    let* i2 = usize_add i 1 in
+    let* slots1 = index_mut_back List_Nil in
+    hashMap_clear_loop t slots1 i2
   else Return slots
 
-(** [hashmap::{hashmap::HashMap<T>}::clear]: merged forward/backward function
-    (there is a single backward function, and the forward function returns ())
+(** [hashmap::{hashmap::HashMap<T>}::clear]:
     Source: 'src/hashmap.rs', lines 80:4-80:27 *)
 let hashMap_clear (t : Type0) (self : hashMap_t t) : result (hashMap_t t) =
-  let* v = hashMap_clear_loop t self.slots 0 in
-  Return { self with num_entries = 0; slots = v }
+  let* back = hashMap_clear_loop t self.slots 0 in
+  Return { self with num_entries = 0; slots = back }
 
-(** [hashmap::{hashmap::HashMap<T>}::len]: forward function
+(** [hashmap::{hashmap::HashMap<T>}::len]:
     Source: 'src/hashmap.rs', lines 90:4-90:30 *)
 let hashMap_len (t : Type0) (self : hashMap_t t) : result usize =
   Return self.num_entries
 
-(** [hashmap::{hashmap::HashMap<T>}::insert_in_list]: loop 0: forward function
+(** [hashmap::{hashmap::HashMap<T>}::insert_in_list]: loop 0:
     Source: 'src/hashmap.rs', lines 97:4-114:5 *)
 let rec hashMap_insert_in_list_loop
   (t : Type0) (key : usize) (value : t) (ls : list_t t) :
-  Tot (result bool)
+  Tot (result (bool & (list_t t)))
   (decreases (hashMap_insert_in_list_loop_decreases t key value ls))
   =
   begin match ls with
   | List_Cons ckey cvalue tl ->
     if ckey = key
-    then Return false
-    else hashMap_insert_in_list_loop t key value tl
-  | List_Nil -> Return true
+    then Return (false, List_Cons ckey value tl)
+    else
+      let* (b, back) = hashMap_insert_in_list_loop t key value tl in
+      Return (b, List_Cons ckey cvalue back)
+  | List_Nil -> let l = List_Nil in Return (true, List_Cons key value l)
   end
 
-(** [hashmap::{hashmap::HashMap<T>}::insert_in_list]: forward function
+(** [hashmap::{hashmap::HashMap<T>}::insert_in_list]:
     Source: 'src/hashmap.rs', lines 97:4-97:71 *)
 let hashMap_insert_in_list
-  (t : Type0) (key : usize) (value : t) (ls : list_t t) : result bool =
+  (t : Type0) (key : usize) (value : t) (ls : list_t t) :
+  result (bool & (list_t t))
+  =
   hashMap_insert_in_list_loop t key value ls
 
-(** [hashmap::{hashmap::HashMap<T>}::insert_in_list]: loop 0: backward function 0
-    Source: 'src/hashmap.rs', lines 97:4-114:5 *)
-let rec hashMap_insert_in_list_loop_back
-  (t : Type0) (key : usize) (value : t) (ls : list_t t) :
-  Tot (result (list_t t))
-  (decreases (hashMap_insert_in_list_loop_decreases t key value ls))
-  =
-  begin match ls with
-  | List_Cons ckey cvalue tl ->
-    if ckey = key
-    then Return (List_Cons ckey value tl)
-    else
-      let* tl0 = hashMap_insert_in_list_loop_back t key value tl in
-      Return (List_Cons ckey cvalue tl0)
-  | List_Nil -> let l = List_Nil in Return (List_Cons key value l)
-  end
-
-(** [hashmap::{hashmap::HashMap<T>}::insert_in_list]: backward function 0
-    Source: 'src/hashmap.rs', lines 97:4-97:71 *)
-let hashMap_insert_in_list_back
-  (t : Type0) (key : usize) (value : t) (ls : list_t t) : result (list_t t) =
-  hashMap_insert_in_list_loop_back t key value ls
-
-(** [hashmap::{hashmap::HashMap<T>}::insert_no_resize]: merged forward/backward function
-    (there is a single backward function, and the forward function returns ())
+(** [hashmap::{hashmap::HashMap<T>}::insert_no_resize]:
     Source: 'src/hashmap.rs', lines 117:4-117:54 *)
 let hashMap_insert_no_resize
   (t : Type0) (self : hashMap_t t) (key : usize) (value : t) :
@@ -143,30 +121,19 @@ let hashMap_insert_no_resize
   let* hash = hash_key key in
   let i = alloc_vec_Vec_len (list_t t) self.slots in
   let* hash_mod = usize_rem hash i in
-  let* l =
+  let* (l, index_mut_back) =
     alloc_vec_Vec_index_mut (list_t t) usize
       (core_slice_index_SliceIndexUsizeSliceTInst (list_t t)) self.slots
       hash_mod in
-  let* inserted = hashMap_insert_in_list t key value l in
+  let* (inserted, l1) = hashMap_insert_in_list t key value l in
   if inserted
   then
-    let* i0 = usize_add self.num_entries 1 in
-    let* l0 = hashMap_insert_in_list_back t key value l in
-    let* v =
-      alloc_vec_Vec_index_mut_back (list_t t) usize
-        (core_slice_index_SliceIndexUsizeSliceTInst (list_t t)) self.slots
-        hash_mod l0 in
-    Return { self with num_entries = i0; slots = v }
-  else
-    let* l0 = hashMap_insert_in_list_back t key value l in
-    let* v =
-      alloc_vec_Vec_index_mut_back (list_t t) usize
-        (core_slice_index_SliceIndexUsizeSliceTInst (list_t t)) self.slots
-        hash_mod l0 in
-    Return { self with slots = v }
+    let* i1 = usize_add self.num_entries 1 in
+    let* v = index_mut_back l1 in
+    Return { self with num_entries = i1; slots = v }
+  else let* v = index_mut_back l1 in Return { self with slots = v }
 
-(** [hashmap::{hashmap::HashMap<T>}::move_elements_from_list]: loop 0: merged forward/backward function
-    (there is a single backward function, and the forward function returns ())
+(** [hashmap::{hashmap::HashMap<T>}::move_elements_from_list]: loop 0:
     Source: 'src/hashmap.rs', lines 183:4-196:5 *)
 let rec hashMap_move_elements_from_list_loop
   (t : Type0) (ntable : hashMap_t t) (ls : list_t t) :
@@ -175,20 +142,18 @@ let rec hashMap_move_elements_from_list_loop
   =
   begin match ls with
   | List_Cons k v tl ->
-    let* ntable0 = hashMap_insert_no_resize t ntable k v in
-    hashMap_move_elements_from_list_loop t ntable0 tl
+    let* hm = hashMap_insert_no_resize t ntable k v in
+    hashMap_move_elements_from_list_loop t hm tl
   | List_Nil -> Return ntable
   end
 
-(** [hashmap::{hashmap::HashMap<T>}::move_elements_from_list]: merged forward/backward function
-    (there is a single backward function, and the forward function returns ())
+(** [hashmap::{hashmap::HashMap<T>}::move_elements_from_list]:
     Source: 'src/hashmap.rs', lines 183:4-183:72 *)
 let hashMap_move_elements_from_list
   (t : Type0) (ntable : hashMap_t t) (ls : list_t t) : result (hashMap_t t) =
   hashMap_move_elements_from_list_loop t ntable ls
 
-(** [hashmap::{hashmap::HashMap<T>}::move_elements]: loop 0: merged forward/backward function
-    (there is a single backward function, and the forward function returns ())
+(** [hashmap::{hashmap::HashMap<T>}::move_elements]: loop 0:
     Source: 'src/hashmap.rs', lines 171:4-180:5 *)
 let rec hashMap_move_elements_loop
   (t : Type0) (ntable : hashMap_t t) (slots : alloc_vec_Vec (list_t t))
@@ -196,64 +161,63 @@ let rec hashMap_move_elements_loop
   Tot (result ((hashMap_t t) & (alloc_vec_Vec (list_t t))))
   (decreases (hashMap_move_elements_loop_decreases t ntable slots i))
   =
-  let i0 = alloc_vec_Vec_len (list_t t) slots in
-  if i < i0
+  let i1 = alloc_vec_Vec_len (list_t t) slots in
+  if i < i1
   then
-    let* l =
+    let* (l, index_mut_back) =
       alloc_vec_Vec_index_mut (list_t t) usize
         (core_slice_index_SliceIndexUsizeSliceTInst (list_t t)) slots i in
-    let ls = core_mem_replace (list_t t) l List_Nil in
-    let* ntable0 = hashMap_move_elements_from_list t ntable ls in
-    let* i1 = usize_add i 1 in
-    let l0 = core_mem_replace_back (list_t t) l List_Nil in
-    let* slots0 =
-      alloc_vec_Vec_index_mut_back (list_t t) usize
-        (core_slice_index_SliceIndexUsizeSliceTInst (list_t t)) slots i l0 in
-    hashMap_move_elements_loop t ntable0 slots0 i1
+    let (ls, l1) = core_mem_replace (list_t t) l List_Nil in
+    let* hm = hashMap_move_elements_from_list t ntable ls in
+    let* i2 = usize_add i 1 in
+    let* slots1 = index_mut_back l1 in
+    let* back_'a = hashMap_move_elements_loop t hm slots1 i2 in
+    let (hm1, v) = back_'a in
+    Return (hm1, v)
   else Return (ntable, slots)
 
-(** [hashmap::{hashmap::HashMap<T>}::move_elements]: merged forward/backward function
-    (there is a single backward function, and the forward function returns ())
+(** [hashmap::{hashmap::HashMap<T>}::move_elements]:
     Source: 'src/hashmap.rs', lines 171:4-171:95 *)
 let hashMap_move_elements
   (t : Type0) (ntable : hashMap_t t) (slots : alloc_vec_Vec (list_t t))
   (i : usize) :
   result ((hashMap_t t) & (alloc_vec_Vec (list_t t)))
   =
-  hashMap_move_elements_loop t ntable slots i
+  let* back_'a = hashMap_move_elements_loop t ntable slots i in
+  let (hm, v) = back_'a in
+  Return (hm, v)
 
-(** [hashmap::{hashmap::HashMap<T>}::try_resize]: merged forward/backward function
-    (there is a single backward function, and the forward function returns ())
+(** [hashmap::{hashmap::HashMap<T>}::try_resize]:
     Source: 'src/hashmap.rs', lines 140:4-140:28 *)
 let hashMap_try_resize
   (t : Type0) (self : hashMap_t t) : result (hashMap_t t) =
   let* max_usize = scalar_cast U32 Usize core_u32_max in
   let capacity = alloc_vec_Vec_len (list_t t) self.slots in
   let* n1 = usize_div max_usize 2 in
-  let (i, i0) = self.max_load_factor in
-  let* i1 = usize_div n1 i in
-  if capacity <= i1
+  let (i, i1) = self.max_load_factor in
+  let* i2 = usize_div n1 i in
+  if capacity <= i2
   then
-    let* i2 = usize_mul capacity 2 in
-    let* ntable = hashMap_new_with_capacity t i2 i i0 in
-    let* (ntable0, _) = hashMap_move_elements t ntable self.slots 0 in
+    let* i3 = usize_mul capacity 2 in
+    let* ntable = hashMap_new_with_capacity t i3 i i1 in
+    let* p = hashMap_move_elements t ntable self.slots 0 in
+    let (ntable1, _) = p in
     Return
-      { ntable0 with num_entries = self.num_entries; max_load_factor = (i, i0)
+      { ntable1 with num_entries = self.num_entries; max_load_factor = (i, i1)
       }
-  else Return { self with max_load_factor = (i, i0) }
+  else Return { self with max_load_factor = (i, i1) }
 
-(** [hashmap::{hashmap::HashMap<T>}::insert]: merged forward/backward function
-    (there is a single backward function, and the forward function returns ())
+(** [hashmap::{hashmap::HashMap<T>}::insert]:
     Source: 'src/hashmap.rs', lines 129:4-129:48 *)
 let hashMap_insert
   (t : Type0) (self : hashMap_t t) (key : usize) (value : t) :
   result (hashMap_t t)
   =
-  let* self0 = hashMap_insert_no_resize t self key value in
-  let* i = hashMap_len t self0 in
-  if i > self0.max_load then hashMap_try_resize t self0 else Return self0
+  let* hm = hashMap_insert_no_resize t self key value in
+  let* i = hashMap_len t hm in
+  if i > hm.max_load then hashMap_try_resize t hm else Return hm
 
-(** [hashmap::{hashmap::HashMap<T>}::contains_key_in_list]: loop 0: forward function
+(** [hashmap::{hashmap::HashMap<T>}::contains_key_in_list]: loop 0:
     Source: 'src/hashmap.rs', lines 206:4-219:5 *)
 let rec hashMap_contains_key_in_list_loop
   (t : Type0) (key : usize) (ls : list_t t) :
@@ -261,20 +225,20 @@ let rec hashMap_contains_key_in_list_loop
   (decreases (hashMap_contains_key_in_list_loop_decreases t key ls))
   =
   begin match ls with
-  | List_Cons ckey x tl ->
+  | List_Cons ckey _ tl ->
     if ckey = key
     then Return true
     else hashMap_contains_key_in_list_loop t key tl
   | List_Nil -> Return false
   end
 
-(** [hashmap::{hashmap::HashMap<T>}::contains_key_in_list]: forward function
+(** [hashmap::{hashmap::HashMap<T>}::contains_key_in_list]:
     Source: 'src/hashmap.rs', lines 206:4-206:68 *)
 let hashMap_contains_key_in_list
   (t : Type0) (key : usize) (ls : list_t t) : result bool =
   hashMap_contains_key_in_list_loop t key ls
 
-(** [hashmap::{hashmap::HashMap<T>}::contains_key]: forward function
+(** [hashmap::{hashmap::HashMap<T>}::contains_key]:
     Source: 'src/hashmap.rs', lines 199:4-199:49 *)
 let hashMap_contains_key
   (t : Type0) (self : hashMap_t t) (key : usize) : result bool =
@@ -287,7 +251,7 @@ let hashMap_contains_key
       hash_mod in
   hashMap_contains_key_in_list t key l
 
-(** [hashmap::{hashmap::HashMap<T>}::get_in_list]: loop 0: forward function
+(** [hashmap::{hashmap::HashMap<T>}::get_in_list]: loop 0:
     Source: 'src/hashmap.rs', lines 224:4-237:5 *)
 let rec hashMap_get_in_list_loop
   (t : Type0) (key : usize) (ls : list_t t) :
@@ -299,12 +263,12 @@ let rec hashMap_get_in_list_loop
   | List_Nil -> Fail Failure
   end
 
-(** [hashmap::{hashmap::HashMap<T>}::get_in_list]: forward function
+(** [hashmap::{hashmap::HashMap<T>}::get_in_list]:
     Source: 'src/hashmap.rs', lines 224:4-224:70 *)
 let hashMap_get_in_list (t : Type0) (key : usize) (ls : list_t t) : result t =
   hashMap_get_in_list_loop t key ls
 
-(** [hashmap::{hashmap::HashMap<T>}::get]: forward function
+(** [hashmap::{hashmap::HashMap<T>}::get]:
     Source: 'src/hashmap.rs', lines 239:4-239:55 *)
 let hashMap_get (t : Type0) (self : hashMap_t t) (key : usize) : result t =
   let* hash = hash_key key in
@@ -316,214 +280,147 @@ let hashMap_get (t : Type0) (self : hashMap_t t) (key : usize) : result t =
       hash_mod in
   hashMap_get_in_list t key l
 
-(** [hashmap::{hashmap::HashMap<T>}::get_mut_in_list]: loop 0: forward function
+(** [hashmap::{hashmap::HashMap<T>}::get_mut_in_list]: loop 0:
     Source: 'src/hashmap.rs', lines 245:4-254:5 *)
 let rec hashMap_get_mut_in_list_loop
   (t : Type0) (ls : list_t t) (key : usize) :
-  Tot (result t) (decreases (hashMap_get_mut_in_list_loop_decreases t ls key))
-  =
-  begin match ls with
-  | List_Cons ckey cvalue tl ->
-    if ckey = key then Return cvalue else hashMap_get_mut_in_list_loop t tl key
-  | List_Nil -> Fail Failure
-  end
-
-(** [hashmap::{hashmap::HashMap<T>}::get_mut_in_list]: forward function
-    Source: 'src/hashmap.rs', lines 245:4-245:86 *)
-let hashMap_get_mut_in_list
-  (t : Type0) (ls : list_t t) (key : usize) : result t =
-  hashMap_get_mut_in_list_loop t ls key
-
-(** [hashmap::{hashmap::HashMap<T>}::get_mut_in_list]: loop 0: backward function 0
-    Source: 'src/hashmap.rs', lines 245:4-254:5 *)
-let rec hashMap_get_mut_in_list_loop_back
-  (t : Type0) (ls : list_t t) (key : usize) (ret : t) :
-  Tot (result (list_t t))
+  Tot (result (t & (t -> result (list_t t))))
   (decreases (hashMap_get_mut_in_list_loop_decreases t ls key))
   =
   begin match ls with
   | List_Cons ckey cvalue tl ->
     if ckey = key
-    then Return (List_Cons ckey ret tl)
+    then
+      let back_'a = fun ret -> Return (List_Cons ckey ret tl) in
+      Return (cvalue, back_'a)
     else
-      let* tl0 = hashMap_get_mut_in_list_loop_back t tl key ret in
-      Return (List_Cons ckey cvalue tl0)
+      let* (x, back_'a) = hashMap_get_mut_in_list_loop t tl key in
+      let back_'a1 =
+        fun ret -> let* tl1 = back_'a ret in Return (List_Cons ckey cvalue tl1)
+        in
+      Return (x, back_'a1)
   | List_Nil -> Fail Failure
   end
 
-(** [hashmap::{hashmap::HashMap<T>}::get_mut_in_list]: backward function 0
+(** [hashmap::{hashmap::HashMap<T>}::get_mut_in_list]:
     Source: 'src/hashmap.rs', lines 245:4-245:86 *)
-let hashMap_get_mut_in_list_back
-  (t : Type0) (ls : list_t t) (key : usize) (ret : t) : result (list_t t) =
-  hashMap_get_mut_in_list_loop_back t ls key ret
+let hashMap_get_mut_in_list
+  (t : Type0) (ls : list_t t) (key : usize) :
+  result (t & (t -> result (list_t t)))
+  =
+  let* (x, back_'a) = hashMap_get_mut_in_list_loop t ls key in
+  let back_'a1 = fun ret -> back_'a ret in
+  Return (x, back_'a1)
 
-(** [hashmap::{hashmap::HashMap<T>}::get_mut]: forward function
+(** [hashmap::{hashmap::HashMap<T>}::get_mut]:
     Source: 'src/hashmap.rs', lines 257:4-257:67 *)
-let hashMap_get_mut (t : Type0) (self : hashMap_t t) (key : usize) : result t =
-  let* hash = hash_key key in
-  let i = alloc_vec_Vec_len (list_t t) self.slots in
-  let* hash_mod = usize_rem hash i in
-  let* l =
-    alloc_vec_Vec_index_mut (list_t t) usize
-      (core_slice_index_SliceIndexUsizeSliceTInst (list_t t)) self.slots
-      hash_mod in
-  hashMap_get_mut_in_list t l key
-
-(** [hashmap::{hashmap::HashMap<T>}::get_mut]: backward function 0
-    Source: 'src/hashmap.rs', lines 257:4-257:67 *)
-let hashMap_get_mut_back
-  (t : Type0) (self : hashMap_t t) (key : usize) (ret : t) :
-  result (hashMap_t t)
+let hashMap_get_mut
+  (t : Type0) (self : hashMap_t t) (key : usize) :
+  result (t & (t -> result (hashMap_t t)))
   =
   let* hash = hash_key key in
   let i = alloc_vec_Vec_len (list_t t) self.slots in
   let* hash_mod = usize_rem hash i in
-  let* l =
+  let* (l, index_mut_back) =
     alloc_vec_Vec_index_mut (list_t t) usize
       (core_slice_index_SliceIndexUsizeSliceTInst (list_t t)) self.slots
       hash_mod in
-  let* l0 = hashMap_get_mut_in_list_back t l key ret in
-  let* v =
-    alloc_vec_Vec_index_mut_back (list_t t) usize
-      (core_slice_index_SliceIndexUsizeSliceTInst (list_t t)) self.slots
-      hash_mod l0 in
-  Return { self with slots = v }
+  let* (x, get_mut_in_list_back) = hashMap_get_mut_in_list t l key in
+  let back_'a =
+    fun ret ->
+      let* l1 = get_mut_in_list_back ret in
+      let* v = index_mut_back l1 in
+      Return { self with slots = v } in
+  Return (x, back_'a)
 
-(** [hashmap::{hashmap::HashMap<T>}::remove_from_list]: loop 0: forward function
+(** [hashmap::{hashmap::HashMap<T>}::remove_from_list]: loop 0:
     Source: 'src/hashmap.rs', lines 265:4-291:5 *)
 let rec hashMap_remove_from_list_loop
   (t : Type0) (key : usize) (ls : list_t t) :
-  Tot (result (option t))
+  Tot (result ((option t) & (list_t t)))
   (decreases (hashMap_remove_from_list_loop_decreases t key ls))
   =
   begin match ls with
   | List_Cons ckey x tl ->
     if ckey = key
     then
-      let mv_ls = core_mem_replace (list_t t) (List_Cons ckey x tl) List_Nil in
+      let (mv_ls, _) =
+        core_mem_replace (list_t t) (List_Cons ckey x tl) List_Nil in
       begin match mv_ls with
-      | List_Cons i cvalue tl0 -> Return (Some cvalue)
-      | List_Nil -> Fail Failure
-      end
-    else hashMap_remove_from_list_loop t key tl
-  | List_Nil -> Return None
-  end
-
-(** [hashmap::{hashmap::HashMap<T>}::remove_from_list]: forward function
-    Source: 'src/hashmap.rs', lines 265:4-265:69 *)
-let hashMap_remove_from_list
-  (t : Type0) (key : usize) (ls : list_t t) : result (option t) =
-  hashMap_remove_from_list_loop t key ls
-
-(** [hashmap::{hashmap::HashMap<T>}::remove_from_list]: loop 0: backward function 1
-    Source: 'src/hashmap.rs', lines 265:4-291:5 *)
-let rec hashMap_remove_from_list_loop_back
-  (t : Type0) (key : usize) (ls : list_t t) :
-  Tot (result (list_t t))
-  (decreases (hashMap_remove_from_list_loop_decreases t key ls))
-  =
-  begin match ls with
-  | List_Cons ckey x tl ->
-    if ckey = key
-    then
-      let mv_ls = core_mem_replace (list_t t) (List_Cons ckey x tl) List_Nil in
-      begin match mv_ls with
-      | List_Cons i cvalue tl0 -> Return tl0
+      | List_Cons _ cvalue tl1 -> Return (Some cvalue, tl1)
       | List_Nil -> Fail Failure
       end
     else
-      let* tl0 = hashMap_remove_from_list_loop_back t key tl in
-      Return (List_Cons ckey x tl0)
-  | List_Nil -> Return List_Nil
+      let* (o, back) = hashMap_remove_from_list_loop t key tl in
+      Return (o, List_Cons ckey x back)
+  | List_Nil -> Return (None, List_Nil)
   end
 
-(** [hashmap::{hashmap::HashMap<T>}::remove_from_list]: backward function 1
+(** [hashmap::{hashmap::HashMap<T>}::remove_from_list]:
     Source: 'src/hashmap.rs', lines 265:4-265:69 *)
-let hashMap_remove_from_list_back
-  (t : Type0) (key : usize) (ls : list_t t) : result (list_t t) =
-  hashMap_remove_from_list_loop_back t key ls
+let hashMap_remove_from_list
+  (t : Type0) (key : usize) (ls : list_t t) :
+  result ((option t) & (list_t t))
+  =
+  hashMap_remove_from_list_loop t key ls
 
-(** [hashmap::{hashmap::HashMap<T>}::remove]: forward function
+(** [hashmap::{hashmap::HashMap<T>}::remove]:
     Source: 'src/hashmap.rs', lines 294:4-294:52 *)
 let hashMap_remove
-  (t : Type0) (self : hashMap_t t) (key : usize) : result (option t) =
+  (t : Type0) (self : hashMap_t t) (key : usize) :
+  result ((option t) & (hashMap_t t))
+  =
   let* hash = hash_key key in
   let i = alloc_vec_Vec_len (list_t t) self.slots in
   let* hash_mod = usize_rem hash i in
-  let* l =
+  let* (l, index_mut_back) =
     alloc_vec_Vec_index_mut (list_t t) usize
       (core_slice_index_SliceIndexUsizeSliceTInst (list_t t)) self.slots
       hash_mod in
-  let* x = hashMap_remove_from_list t key l in
-  begin match x with
-  | None -> Return None
-  | Some x0 -> let* _ = usize_sub self.num_entries 1 in Return (Some x0)
-  end
-
-(** [hashmap::{hashmap::HashMap<T>}::remove]: backward function 0
-    Source: 'src/hashmap.rs', lines 294:4-294:52 *)
-let hashMap_remove_back
-  (t : Type0) (self : hashMap_t t) (key : usize) : result (hashMap_t t) =
-  let* hash = hash_key key in
-  let i = alloc_vec_Vec_len (list_t t) self.slots in
-  let* hash_mod = usize_rem hash i in
-  let* l =
-    alloc_vec_Vec_index_mut (list_t t) usize
-      (core_slice_index_SliceIndexUsizeSliceTInst (list_t t)) self.slots
-      hash_mod in
-  let* x = hashMap_remove_from_list t key l in
+  let* (x, l1) = hashMap_remove_from_list t key l in
   begin match x with
   | None ->
-    let* l0 = hashMap_remove_from_list_back t key l in
-    let* v =
-      alloc_vec_Vec_index_mut_back (list_t t) usize
-        (core_slice_index_SliceIndexUsizeSliceTInst (list_t t)) self.slots
-        hash_mod l0 in
-    Return { self with slots = v }
-  | Some x0 ->
-    let* i0 = usize_sub self.num_entries 1 in
-    let* l0 = hashMap_remove_from_list_back t key l in
-    let* v =
-      alloc_vec_Vec_index_mut_back (list_t t) usize
-        (core_slice_index_SliceIndexUsizeSliceTInst (list_t t)) self.slots
-        hash_mod l0 in
-    Return { self with num_entries = i0; slots = v }
+    let* v = index_mut_back l1 in Return (None, { self with slots = v })
+  | Some x1 ->
+    let* i1 = usize_sub self.num_entries 1 in
+    let* v = index_mut_back l1 in
+    Return (Some x1, { self with num_entries = i1; slots = v })
   end
 
-(** [hashmap::test1]: forward function
+(** [hashmap::test1]:
     Source: 'src/hashmap.rs', lines 315:0-315:10 *)
 let test1 : result unit =
   let* hm = hashMap_new u64 in
-  let* hm0 = hashMap_insert u64 hm 0 42 in
-  let* hm1 = hashMap_insert u64 hm0 128 18 in
-  let* hm2 = hashMap_insert u64 hm1 1024 138 in
-  let* hm3 = hashMap_insert u64 hm2 1056 256 in
-  let* i = hashMap_get u64 hm3 128 in
+  let* hm1 = hashMap_insert u64 hm 0 42 in
+  let* hm2 = hashMap_insert u64 hm1 128 18 in
+  let* hm3 = hashMap_insert u64 hm2 1024 138 in
+  let* hm4 = hashMap_insert u64 hm3 1056 256 in
+  let* i = hashMap_get u64 hm4 128 in
   if not (i = 18)
   then Fail Failure
   else
-    let* hm4 = hashMap_get_mut_back u64 hm3 1024 56 in
-    let* i0 = hashMap_get u64 hm4 1024 in
-    if not (i0 = 56)
+    let* (_, get_mut_back) = hashMap_get_mut u64 hm4 1024 in
+    let* hm5 = get_mut_back 56 in
+    let* i1 = hashMap_get u64 hm5 1024 in
+    if not (i1 = 56)
     then Fail Failure
     else
-      let* x = hashMap_remove u64 hm4 1024 in
+      let* (x, hm6) = hashMap_remove u64 hm5 1024 in
       begin match x with
       | None -> Fail Failure
-      | Some x0 ->
-        if not (x0 = 56)
+      | Some x1 ->
+        if not (x1 = 56)
         then Fail Failure
         else
-          let* hm5 = hashMap_remove_back u64 hm4 1024 in
-          let* i1 = hashMap_get u64 hm5 0 in
-          if not (i1 = 42)
+          let* i2 = hashMap_get u64 hm6 0 in
+          if not (i2 = 42)
           then Fail Failure
           else
-            let* i2 = hashMap_get u64 hm5 128 in
-            if not (i2 = 18)
+            let* i3 = hashMap_get u64 hm6 128 in
+            if not (i3 = 18)
             then Fail Failure
             else
-              let* i3 = hashMap_get u64 hm5 1056 in
-              if not (i3 = 256) then Fail Failure else Return ()
+              let* i4 = hashMap_get u64 hm6 1056 in
+              if not (i4 = 256) then Fail Failure else Return ()
       end
 
