tests/fstar/misc/Paper.fst
@@ -5,40 +5,36 @@ open Primitives
 
 #set-options "--z3rlimit 50 --fuel 1 --ifuel 1"
 
-(** [paper::ref_incr]: merged forward/backward function
-    (there is a single backward function, and the forward function returns ())
+(** [paper::ref_incr]:
     Source: 'src/paper.rs', lines 4:0-4:28 *)
 let ref_incr (x : i32) : result i32 =
   i32_add x 1
 
-(** [paper::test_incr]: forward function
+(** [paper::test_incr]:
     Source: 'src/paper.rs', lines 8:0-8:18 *)
 let test_incr : result unit =
-  let* x = ref_incr 0 in if not (x = 1) then Fail Failure else Return ()
+  let* i = ref_incr 0 in if not (i = 1) then Fail Failure else Return ()
 
 (** Unit test for [paper::test_incr] *)
 let _ = assert_norm (test_incr = Return ())
 
-(** [paper::choose]: forward function
+(** [paper::choose]:
     Source: 'src/paper.rs', lines 15:0-15:70 *)
-let choose (t : Type0) (b : bool) (x : t) (y : t) : result t =
-  if b then Return x else Return y
+let choose
+  (t : Type0) (b : bool) (x : t) (y : t) : result (t & (t -> result (t & t))) =
+  if b
+  then let back_'a = fun ret -> Return (ret, y) in Return (x, back_'a)
+  else let back_'a = fun ret -> Return (x, ret) in Return (y, back_'a)
 
-(** [paper::choose]: backward function 0
-    Source: 'src/paper.rs', lines 15:0-15:70 *)
-let choose_back
-  (t : Type0) (b : bool) (x : t) (y : t) (ret : t) : result (t & t) =
-  if b then Return (ret, y) else Return (x, ret)
-
-(** [paper::test_choose]: forward function
+(** [paper::test_choose]:
     Source: 'src/paper.rs', lines 23:0-23:20 *)
 let test_choose : result unit =
-  let* z = choose i32 true 0 0 in
-  let* z0 = i32_add z 1 in
-  if not (z0 = 1)
+  let* (z, choose_back) = choose i32 true 0 0 in
+  let* z1 = i32_add z 1 in
+  if not (z1 = 1)
   then Fail Failure
   else
-    let* (x, y) = choose_back i32 true 0 0 z0 in
+    let* (x, y) = choose_back z1 in
     if not (x = 1)
     then Fail Failure
     else if not (y = 0) then Fail Failure else Return ()
@@ -52,31 +48,28 @@ type list_t (t : Type0) =
 | List_Cons : t -> list_t t -> list_t t
 | List_Nil : list_t t
 
-(** [paper::list_nth_mut]: forward function
+(** [paper::list_nth_mut]:
     Source: 'src/paper.rs', lines 42:0-42:67 *)
-let rec list_nth_mut (t : Type0) (l : list_t t) (i : u32) : result t =
-  begin match l with
-  | List_Cons x tl ->
-    if i = 0 then Return x else let* i0 = u32_sub i 1 in list_nth_mut t tl i0
-  | List_Nil -> Fail Failure
-  end
-
-(** [paper::list_nth_mut]: backward function 0
-    Source: 'src/paper.rs', lines 42:0-42:67 *)
-let rec list_nth_mut_back
-  (t : Type0) (l : list_t t) (i : u32) (ret : t) : result (list_t t) =
+let rec list_nth_mut
+  (t : Type0) (l : list_t t) (i : u32) :
+  result (t & (t -> result (list_t t)))
+  =
   begin match l with
   | List_Cons x tl ->
     if i = 0
-    then Return (List_Cons ret tl)
+    then
+      let back_'a = fun ret -> Return (List_Cons ret tl) in Return (x, back_'a)
     else
-      let* i0 = u32_sub i 1 in
-      let* tl0 = list_nth_mut_back t tl i0 ret in
-      Return (List_Cons x tl0)
+      let* i1 = u32_sub i 1 in
+      let* (x1, list_nth_mut_back) = list_nth_mut t tl i1 in
+      let back_'a =
+        fun ret -> let* tl1 = list_nth_mut_back ret in Return (List_Cons x tl1)
+        in
+      Return (x1, back_'a)
   | List_Nil -> Fail Failure
   end
 
-(** [paper::sum]: forward function
+(** [paper::sum]:
     Source: 'src/paper.rs', lines 57:0-57:32 *)
 let rec sum (l : list_t i32) : result i32 =
   begin match l with
@@ -84,27 +77,27 @@ let rec sum (l : list_t i32) : result i32 =
   | List_Nil -> Return 0
   end
 
-(** [paper::test_nth]: forward function
+(** [paper::test_nth]:
     Source: 'src/paper.rs', lines 68:0-68:17 *)
 let test_nth : result unit =
   let l = List_Nil in
-  let l0 = List_Cons 3 l in
-  let l1 = List_Cons 2 l0 in
-  let* x = list_nth_mut i32 (List_Cons 1 l1) 2 in
-  let* x0 = i32_add x 1 in
-  let* l2 = list_nth_mut_back i32 (List_Cons 1 l1) 2 x0 in
-  let* i = sum l2 in
+  let l1 = List_Cons 3 l in
+  let l2 = List_Cons 2 l1 in
+  let* (x, list_nth_mut_back) = list_nth_mut i32 (List_Cons 1 l2) 2 in
+  let* x1 = i32_add x 1 in
+  let* l3 = list_nth_mut_back x1 in
+  let* i = sum l3 in
   if not (i = 7) then Fail Failure else Return ()
 
 (** Unit test for [paper::test_nth] *)
 let _ = assert_norm (test_nth = Return ())
 
-(** [paper::call_choose]: forward function
+(** [paper::call_choose]:
     Source: 'src/paper.rs', lines 76:0-76:44 *)
 let call_choose (p : (u32 & u32)) : result u32 =
   let (px, py) = p in
-  let* pz = choose u32 true px py in
-  let* pz0 = u32_add pz 1 in
-  let* (px0, _) = choose_back u32 true px py pz0 in
-  Return px0
+  let* (pz, choose_back) = choose u32 true px py in
+  let* pz1 = u32_add pz 1 in
+  let* (px1, _) = choose_back pz1 in
+  Return px1
 
