tests/lean/Loops.lean
@@ -5,73 +5,72 @@ open Primitives
 
 namespace loops
 
-/- [loops::sum]: loop 0: forward function
+/- [loops::sum]: loop 0:
    Source: 'src/loops.rs', lines 4:0-14:1 -/
 divergent def sum_loop (max : U32) (i : U32) (s : U32) : Result U32 :=
   if i < max
   then do
-         let s0 ← s + i
-         let i0 ← i + 1#u32
-         sum_loop max i0 s0
+       let s1 ← s + i
+       let i1 ← i + 1#u32
+       sum_loop max i1 s1
   else s * 2#u32
 
-/- [loops::sum]: forward function
+/- [loops::sum]:
    Source: 'src/loops.rs', lines 4:0-4:27 -/
 def sum (max : U32) : Result U32 :=
   sum_loop max 0#u32 0#u32
 
-/- [loops::sum_with_mut_borrows]: loop 0: forward function
+/- [loops::sum_with_mut_borrows]: loop 0:
    Source: 'src/loops.rs', lines 19:0-31:1 -/
 divergent def sum_with_mut_borrows_loop
   (max : U32) (mi : U32) (ms : U32) : Result U32 :=
   if mi < max
   then
     do
-      let ms0 ← ms + mi
-      let mi0 ← mi + 1#u32
-      sum_with_mut_borrows_loop max mi0 ms0
+    let ms1 ← ms + mi
+    let mi1 ← mi + 1#u32
+    sum_with_mut_borrows_loop max mi1 ms1
   else ms * 2#u32
 
-/- [loops::sum_with_mut_borrows]: forward function
+/- [loops::sum_with_mut_borrows]:
    Source: 'src/loops.rs', lines 19:0-19:44 -/
 def sum_with_mut_borrows (max : U32) : Result U32 :=
   sum_with_mut_borrows_loop max 0#u32 0#u32
 
-/- [loops::sum_with_shared_borrows]: loop 0: forward function
+/- [loops::sum_with_shared_borrows]: loop 0:
    Source: 'src/loops.rs', lines 34:0-48:1 -/
 divergent def sum_with_shared_borrows_loop
   (max : U32) (i : U32) (s : U32) : Result U32 :=
   if i < max
   then
     do
-      let i0 ← i + 1#u32
-      let s0 ← s + i0
-      sum_with_shared_borrows_loop max i0 s0
+    let i1 ← i + 1#u32
+    let s1 ← s + i1
+    sum_with_shared_borrows_loop max i1 s1
   else s * 2#u32
 
-/- [loops::sum_with_shared_borrows]: forward function
+/- [loops::sum_with_shared_borrows]:
    Source: 'src/loops.rs', lines 34:0-34:47 -/
 def sum_with_shared_borrows (max : U32) : Result U32 :=
   sum_with_shared_borrows_loop max 0#u32 0#u32
 
-/- [loops::clear]: loop 0: merged forward/backward function
-   (there is a single backward function, and the forward function returns ())
+/- [loops::clear]: loop 0:
    Source: 'src/loops.rs', lines 52:0-58:1 -/
 divergent def clear_loop
   (v : alloc.vec.Vec U32) (i : Usize) : Result (alloc.vec.Vec U32) :=
-  let i0 := alloc.vec.Vec.len U32 v
-  if i < i0
+  let i1 := alloc.vec.Vec.len U32 v
+  if i < i1
   then
     do
-      let i1 ← i + 1#usize
-      let v0 ←
-        alloc.vec.Vec.index_mut_back U32 Usize
-          (core.slice.index.SliceIndexUsizeSliceTInst U32) v i 0#u32
-      clear_loop v0 i1
+    let (_, index_mut_back) ←
+      alloc.vec.Vec.index_mut U32 Usize
+        (core.slice.index.SliceIndexUsizeSliceTInst U32) v i
+    let i2 ← i + 1#usize
+    let v1 ← index_mut_back 0#u32
+    clear_loop v1 i2
   else Result.ret v
 
-/- [loops::clear]: merged forward/backward function
-   (there is a single backward function, and the forward function returns ())
+/- [loops::clear]:
    Source: 'src/loops.rs', lines 52:0-52:30 -/
 def clear (v : alloc.vec.Vec U32) : Result (alloc.vec.Vec U32) :=
   clear_loop v 0#usize
@@ -82,7 +81,7 @@ inductive List (T : Type) :=
 | Cons : T → List T → List T
 | Nil : List T
 
-/- [loops::list_mem]: loop 0: forward function
+/- [loops::list_mem]: loop 0:
    Source: 'src/loops.rs', lines 66:0-75:1 -/
 divergent def list_mem_loop (x : U32) (ls : List U32) : Result Bool :=
   match ls with
@@ -91,51 +90,42 @@ divergent def list_mem_loop (x : U32) (ls : List U32) : Result Bool :=
                       else list_mem_loop x tl
   | List.Nil => Result.ret false
 
-/- [loops::list_mem]: forward function
+/- [loops::list_mem]:
    Source: 'src/loops.rs', lines 66:0-66:52 -/
 def list_mem (x : U32) (ls : List U32) : Result Bool :=
   list_mem_loop x ls
 
-/- [loops::list_nth_mut_loop]: loop 0: forward function
+/- [loops::list_nth_mut_loop]: loop 0:
    Source: 'src/loops.rs', lines 78:0-88:1 -/
 divergent def list_nth_mut_loop_loop
-  (T : Type) (ls : List T) (i : U32) : Result T :=
+  (T : Type) (ls : List T) (i : U32) : Result (T × (T → Result (List T))) :=
   match ls with
   | List.Cons x tl =>
     if i = 0#u32
-    then Result.ret x
-    else do
-           let i0 ← i - 1#u32
-           list_nth_mut_loop_loop T tl i0
-  | List.Nil => Result.fail .panic
-
-/- [loops::list_nth_mut_loop]: forward function
-   Source: 'src/loops.rs', lines 78:0-78:71 -/
-def list_nth_mut_loop (T : Type) (ls : List T) (i : U32) : Result T :=
-  list_nth_mut_loop_loop T ls i
-
-/- [loops::list_nth_mut_loop]: loop 0: backward function 0
-   Source: 'src/loops.rs', lines 78:0-88:1 -/
-divergent def list_nth_mut_loop_loop_back
-  (T : Type) (ls : List T) (i : U32) (ret : T) : Result (List T) :=
-  match ls with
-  | List.Cons x tl =>
-    if i = 0#u32
-    then Result.ret (List.Cons ret tl)
+    then
+      let back := fun ret => Result.ret (List.Cons ret tl)
+      Result.ret (x, back)
     else
       do
-        let i0 ← i - 1#u32
-        let tl0 ← list_nth_mut_loop_loop_back T tl i0 ret
-        Result.ret (List.Cons x tl0)
+      let i1 ← i - 1#u32
+      let (t, back) ← list_nth_mut_loop_loop T tl i1
+      let back1 :=
+        fun ret => do
+                   let tl1 ← back ret
+                   Result.ret (List.Cons x tl1)
+      Result.ret (t, back1)
   | List.Nil => Result.fail .panic
 
-/- [loops::list_nth_mut_loop]: backward function 0
+/- [loops::list_nth_mut_loop]:
    Source: 'src/loops.rs', lines 78:0-78:71 -/
-def list_nth_mut_loop_back
-  (T : Type) (ls : List T) (i : U32) (ret : T) : Result (List T) :=
-  list_nth_mut_loop_loop_back T ls i ret
+def list_nth_mut_loop
+  (T : Type) (ls : List T) (i : U32) : Result (T × (T → Result (List T))) :=
+  do
+  let (t, back) ← list_nth_mut_loop_loop T ls i
+  let back1 := fun ret => back ret
+  Result.ret (t, back1)
 
-/- [loops::list_nth_shared_loop]: loop 0: forward function
+/- [loops::list_nth_shared_loop]: loop 0:
    Source: 'src/loops.rs', lines 91:0-101:1 -/
 divergent def list_nth_shared_loop_loop
   (T : Type) (ls : List T) (i : U32) : Result T :=
@@ -144,64 +134,54 @@ divergent def list_nth_shared_loop_loop
     if i = 0#u32
     then Result.ret x
     else do
-           let i0 ← i - 1#u32
-           list_nth_shared_loop_loop T tl i0
+         let i1 ← i - 1#u32
+         list_nth_shared_loop_loop T tl i1
   | List.Nil => Result.fail .panic
 
-/- [loops::list_nth_shared_loop]: forward function
+/- [loops::list_nth_shared_loop]:
    Source: 'src/loops.rs', lines 91:0-91:66 -/
 def list_nth_shared_loop (T : Type) (ls : List T) (i : U32) : Result T :=
   list_nth_shared_loop_loop T ls i
 
-/- [loops::get_elem_mut]: loop 0: forward function
+/- [loops::get_elem_mut]: loop 0:
    Source: 'src/loops.rs', lines 103:0-117:1 -/
-divergent def get_elem_mut_loop (x : Usize) (ls : List Usize) : Result Usize :=
-  match ls with
-  | List.Cons y tl => if y = x
-                      then Result.ret y
-                      else get_elem_mut_loop x tl
-  | List.Nil => Result.fail .panic
-
-/- [loops::get_elem_mut]: forward function
-   Source: 'src/loops.rs', lines 103:0-103:73 -/
-def get_elem_mut
-  (slots : alloc.vec.Vec (List Usize)) (x : Usize) : Result Usize :=
-  do
-    let l ←
-      alloc.vec.Vec.index_mut (List Usize) Usize
-        (core.slice.index.SliceIndexUsizeSliceTInst (List Usize)) slots 0#usize
-    get_elem_mut_loop x l
-
-/- [loops::get_elem_mut]: loop 0: backward function 0
-   Source: 'src/loops.rs', lines 103:0-117:1 -/
-divergent def get_elem_mut_loop_back
-  (x : Usize) (ls : List Usize) (ret : Usize) : Result (List Usize) :=
+divergent def get_elem_mut_loop
+  (x : Usize) (ls : List Usize) :
+  Result (Usize × (Usize → Result (List Usize)))
+  :=
   match ls with
   | List.Cons y tl =>
     if y = x
-    then Result.ret (List.Cons ret tl)
+    then
+      let back := fun ret => Result.ret (List.Cons ret tl)
+      Result.ret (y, back)
     else
       do
-        let tl0 ← get_elem_mut_loop_back x tl ret
-        Result.ret (List.Cons y tl0)
+      let (i, back) ← get_elem_mut_loop x tl
+      let back1 :=
+        fun ret => do
+                   let tl1 ← back ret
+                   Result.ret (List.Cons y tl1)
+      Result.ret (i, back1)
   | List.Nil => Result.fail .panic
 
-/- [loops::get_elem_mut]: backward function 0
+/- [loops::get_elem_mut]:
    Source: 'src/loops.rs', lines 103:0-103:73 -/
-def get_elem_mut_back
-  (slots : alloc.vec.Vec (List Usize)) (x : Usize) (ret : Usize) :
-  Result (alloc.vec.Vec (List Usize))
+def get_elem_mut
+  (slots : alloc.vec.Vec (List Usize)) (x : Usize) :
+  Result (Usize × (Usize → Result (alloc.vec.Vec (List Usize))))
   :=
   do
-    let l ←
-      alloc.vec.Vec.index_mut (List Usize) Usize
-        (core.slice.index.SliceIndexUsizeSliceTInst (List Usize)) slots 0#usize
-    let l0 ← get_elem_mut_loop_back x l ret
-    alloc.vec.Vec.index_mut_back (List Usize) Usize
+  let (l, index_mut_back) ←
+    alloc.vec.Vec.index_mut (List Usize) Usize
       (core.slice.index.SliceIndexUsizeSliceTInst (List Usize)) slots 0#usize
-      l0
+  let (i, back) ← get_elem_mut_loop x l
+  let back1 := fun ret => do
+                          let l1 ← back ret
+                          index_mut_back l1
+  Result.ret (i, back1)
 
-/- [loops::get_elem_shared]: loop 0: forward function
+/- [loops::get_elem_shared]: loop 0:
    Source: 'src/loops.rs', lines 119:0-133:1 -/
 divergent def get_elem_shared_loop
   (x : Usize) (ls : List Usize) : Result Usize :=
@@ -211,76 +191,64 @@ divergent def get_elem_shared_loop
                       else get_elem_shared_loop x tl
   | List.Nil => Result.fail .panic
 
-/- [loops::get_elem_shared]: forward function
+/- [loops::get_elem_shared]:
    Source: 'src/loops.rs', lines 119:0-119:68 -/
 def get_elem_shared
   (slots : alloc.vec.Vec (List Usize)) (x : Usize) : Result Usize :=
   do
-    let l ←
-      alloc.vec.Vec.index (List Usize) Usize
-        (core.slice.index.SliceIndexUsizeSliceTInst (List Usize)) slots 0#usize
-    get_elem_shared_loop x l
+  let l ←
+    alloc.vec.Vec.index (List Usize) Usize
+      (core.slice.index.SliceIndexUsizeSliceTInst (List Usize)) slots 0#usize
+  get_elem_shared_loop x l
 
-/- [loops::id_mut]: forward function
+/- [loops::id_mut]:
    Source: 'src/loops.rs', lines 135:0-135:50 -/
-def id_mut (T : Type) (ls : List T) : Result (List T) :=
-  Result.ret ls
+def id_mut
+  (T : Type) (ls : List T) :
+  Result ((List T) × (List T → Result (List T)))
+  :=
+  let back := fun ret => Result.ret ret
+  Result.ret (ls, back)
 
-/- [loops::id_mut]: backward function 0
-   Source: 'src/loops.rs', lines 135:0-135:50 -/
-def id_mut_back (T : Type) (ls : List T) (ret : List T) : Result (List T) :=
-  Result.ret ret
-
-/- [loops::id_shared]: forward function
+/- [loops::id_shared]:
    Source: 'src/loops.rs', lines 139:0-139:45 -/
 def id_shared (T : Type) (ls : List T) : Result (List T) :=
   Result.ret ls
 
-/- [loops::list_nth_mut_loop_with_id]: loop 0: forward function
+/- [loops::list_nth_mut_loop_with_id]: loop 0:
    Source: 'src/loops.rs', lines 144:0-155:1 -/
 divergent def list_nth_mut_loop_with_id_loop
-  (T : Type) (i : U32) (ls : List T) : Result T :=
+  (T : Type) (i : U32) (ls : List T) : Result (T × (T → Result (List T))) :=
   match ls with
   | List.Cons x tl =>
     if i = 0#u32
-    then Result.ret x
-    else do
-           let i0 ← i - 1#u32
-           list_nth_mut_loop_with_id_loop T i0 tl
-  | List.Nil => Result.fail .panic
-
-/- [loops::list_nth_mut_loop_with_id]: forward function
-   Source: 'src/loops.rs', lines 144:0-144:75 -/
-def list_nth_mut_loop_with_id (T : Type) (ls : List T) (i : U32) : Result T :=
-  do
-    let ls0 ← id_mut T ls
-    list_nth_mut_loop_with_id_loop T i ls0
-
-/- [loops::list_nth_mut_loop_with_id]: loop 0: backward function 0
-   Source: 'src/loops.rs', lines 144:0-155:1 -/
-divergent def list_nth_mut_loop_with_id_loop_back
-  (T : Type) (i : U32) (ls : List T) (ret : T) : Result (List T) :=
-  match ls with
-  | List.Cons x tl =>
-    if i = 0#u32
-    then Result.ret (List.Cons ret tl)
+    then
+      let back := fun ret => Result.ret (List.Cons ret tl)
+      Result.ret (x, back)
     else
       do
-        let i0 ← i - 1#u32
-        let tl0 ← list_nth_mut_loop_with_id_loop_back T i0 tl ret
-        Result.ret (List.Cons x tl0)
+      let i1 ← i - 1#u32
+      let (t, back) ← list_nth_mut_loop_with_id_loop T i1 tl
+      let back1 :=
+        fun ret => do
+                   let tl1 ← back ret
+                   Result.ret (List.Cons x tl1)
+      Result.ret (t, back1)
   | List.Nil => Result.fail .panic
 
-/- [loops::list_nth_mut_loop_with_id]: backward function 0
+/- [loops::list_nth_mut_loop_with_id]:
    Source: 'src/loops.rs', lines 144:0-144:75 -/
-def list_nth_mut_loop_with_id_back
-  (T : Type) (ls : List T) (i : U32) (ret : T) : Result (List T) :=
+def list_nth_mut_loop_with_id
+  (T : Type) (ls : List T) (i : U32) : Result (T × (T → Result (List T))) :=
   do
-    let ls0 ← id_mut T ls
-    let l ← list_nth_mut_loop_with_id_loop_back T i ls0 ret
-    id_mut_back T ls l
+  let (ls1, id_mut_back) ← id_mut T ls
+  let (t, back) ← list_nth_mut_loop_with_id_loop T i ls1
+  let back1 := fun ret => do
+                          let l ← back ret
+                          id_mut_back l
+  Result.ret (t, back1)
 
-/- [loops::list_nth_shared_loop_with_id]: loop 0: forward function
+/- [loops::list_nth_shared_loop_with_id]: loop 0:
    Source: 'src/loops.rs', lines 158:0-169:1 -/
 divergent def list_nth_shared_loop_with_id_loop
   (T : Type) (i : U32) (ls : List T) : Result T :=
@@ -289,97 +257,62 @@ divergent def list_nth_shared_loop_with_id_loop
     if i = 0#u32
     then Result.ret x
     else do
-           let i0 ← i - 1#u32
-           list_nth_shared_loop_with_id_loop T i0 tl
+         let i1 ← i - 1#u32
+         list_nth_shared_loop_with_id_loop T i1 tl
   | List.Nil => Result.fail .panic
 
-/- [loops::list_nth_shared_loop_with_id]: forward function
+/- [loops::list_nth_shared_loop_with_id]:
    Source: 'src/loops.rs', lines 158:0-158:70 -/
 def list_nth_shared_loop_with_id
   (T : Type) (ls : List T) (i : U32) : Result T :=
   do
-    let ls0 ← id_shared T ls
-    list_nth_shared_loop_with_id_loop T i ls0
+  let ls1 ← id_shared T ls
+  list_nth_shared_loop_with_id_loop T i ls1
 
-/- [loops::list_nth_mut_loop_pair]: loop 0: forward function
+/- [loops::list_nth_mut_loop_pair]: loop 0:
    Source: 'src/loops.rs', lines 174:0-195:1 -/
 divergent def list_nth_mut_loop_pair_loop
-  (T : Type) (ls0 : List T) (ls1 : List T) (i : U32) : Result (T × T) :=
+  (T : Type) (ls0 : List T) (ls1 : List T) (i : U32) :
+  Result ((T × T) × (T → Result (List T)) × (T → Result (List T)))
+  :=
   match ls0 with
   | List.Cons x0 tl0 =>
     match ls1 with
     | List.Cons x1 tl1 =>
       if i = 0#u32
-      then Result.ret (x0, x1)
-      else do
-             let i0 ← i - 1#u32
-             list_nth_mut_loop_pair_loop T tl0 tl1 i0
+      then
+        let back_'a := fun ret => Result.ret (List.Cons ret tl0)
+        let back_'b := fun ret => Result.ret (List.Cons ret tl1)
+        Result.ret ((x0, x1), back_'a, back_'b)
+      else
+        do
+        let i1 ← i - 1#u32
+        let (p, back_'a, back_'b) ← list_nth_mut_loop_pair_loop T tl0 tl1 i1
+        let back_'a1 :=
+          fun ret => do
+                     let tl01 ← back_'a ret
+                     Result.ret (List.Cons x0 tl01)
+        let back_'b1 :=
+          fun ret => do
+                     let tl11 ← back_'b ret
+                     Result.ret (List.Cons x1 tl11)
+        Result.ret (p, back_'a1, back_'b1)
     | List.Nil => Result.fail .panic
   | List.Nil => Result.fail .panic
 
-/- [loops::list_nth_mut_loop_pair]: forward function
+/- [loops::list_nth_mut_loop_pair]:
    Source: 'src/loops.rs', lines 174:0-178:27 -/
 def list_nth_mut_loop_pair
-  (T : Type) (ls0 : List T) (ls1 : List T) (i : U32) : Result (T × T) :=
-  list_nth_mut_loop_pair_loop T ls0 ls1 i
-
-/- [loops::list_nth_mut_loop_pair]: loop 0: backward function 0
-   Source: 'src/loops.rs', lines 174:0-195:1 -/
-divergent def list_nth_mut_loop_pair_loop_back'a
-  (T : Type) (ls0 : List T) (ls1 : List T) (i : U32) (ret : T) :
-  Result (List T)
+  (T : Type) (ls0 : List T) (ls1 : List T) (i : U32) :
+  Result ((T × T) × (T → Result (List T)) × (T → Result (List T)))
   :=
-  match ls0 with
-  | List.Cons x0 tl0 =>
-    match ls1 with
-    | List.Cons x1 tl1 =>
-      if i = 0#u32
-      then Result.ret (List.Cons ret tl0)
-      else
-        do
-          let i0 ← i - 1#u32
-          let tl00 ← list_nth_mut_loop_pair_loop_back'a T tl0 tl1 i0 ret
-          Result.ret (List.Cons x0 tl00)
-    | List.Nil => Result.fail .panic
-  | List.Nil => Result.fail .panic
+  do
+  let (p, back_'a, back_'b) ← list_nth_mut_loop_pair_loop T ls0 ls1 i
+  let back_'a1 := fun ret => back_'a ret
+  let back_'b1 := fun ret => back_'b ret
+  Result.ret (p, back_'a1, back_'b1)
 
-/- [loops::list_nth_mut_loop_pair]: backward function 0
-   Source: 'src/loops.rs', lines 174:0-178:27 -/
-def list_nth_mut_loop_pair_back'a
-  (T : Type) (ls0 : List T) (ls1 : List T) (i : U32) (ret : T) :
-  Result (List T)
-  :=
-  list_nth_mut_loop_pair_loop_back'a T ls0 ls1 i ret
-
-/- [loops::list_nth_mut_loop_pair]: loop 0: backward function 1
-   Source: 'src/loops.rs', lines 174:0-195:1 -/
-divergent def list_nth_mut_loop_pair_loop_back'b
-  (T : Type) (ls0 : List T) (ls1 : List T) (i : U32) (ret : T) :
-  Result (List T)
-  :=
-  match ls0 with
-  | List.Cons x0 tl0 =>
-    match ls1 with
-    | List.Cons x1 tl1 =>
-      if i = 0#u32
-      then Result.ret (List.Cons ret tl1)
-      else
-        do
-          let i0 ← i - 1#u32
-          let tl10 ← list_nth_mut_loop_pair_loop_back'b T tl0 tl1 i0 ret
-          Result.ret (List.Cons x1 tl10)
-    | List.Nil => Result.fail .panic
-  | List.Nil => Result.fail .panic
-
-/- [loops::list_nth_mut_loop_pair]: backward function 1
-   Source: 'src/loops.rs', lines 174:0-178:27 -/
-def list_nth_mut_loop_pair_back'b
-  (T : Type) (ls0 : List T) (ls1 : List T) (i : U32) (ret : T) :
-  Result (List T)
-  :=
-  list_nth_mut_loop_pair_loop_back'b T ls0 ls1 i ret
-
-/- [loops::list_nth_shared_loop_pair]: loop 0: forward function
+/- [loops::list_nth_shared_loop_pair]: loop 0:
    Source: 'src/loops.rs', lines 198:0-219:1 -/
 divergent def list_nth_shared_loop_pair_loop
   (T : Type) (ls0 : List T) (ls1 : List T) (i : U32) : Result (T × T) :=
@@ -390,71 +323,59 @@ divergent def list_nth_shared_loop_pair_loop
       if i = 0#u32
       then Result.ret (x0, x1)
       else do
-             let i0 ← i - 1#u32
-             list_nth_shared_loop_pair_loop T tl0 tl1 i0
+           let i1 ← i - 1#u32
+           list_nth_shared_loop_pair_loop T tl0 tl1 i1
     | List.Nil => Result.fail .panic
   | List.Nil => Result.fail .panic
 
-/- [loops::list_nth_shared_loop_pair]: forward function
+/- [loops::list_nth_shared_loop_pair]:
    Source: 'src/loops.rs', lines 198:0-202:19 -/
 def list_nth_shared_loop_pair
   (T : Type) (ls0 : List T) (ls1 : List T) (i : U32) : Result (T × T) :=
   list_nth_shared_loop_pair_loop T ls0 ls1 i
 
-/- [loops::list_nth_mut_loop_pair_merge]: loop 0: forward function
+/- [loops::list_nth_mut_loop_pair_merge]: loop 0:
    Source: 'src/loops.rs', lines 223:0-238:1 -/
 divergent def list_nth_mut_loop_pair_merge_loop
-  (T : Type) (ls0 : List T) (ls1 : List T) (i : U32) : Result (T × T) :=
+  (T : Type) (ls0 : List T) (ls1 : List T) (i : U32) :
+  Result ((T × T) × ((T × T) → Result ((List T) × (List T))))
+  :=
   match ls0 with
   | List.Cons x0 tl0 =>
     match ls1 with
     | List.Cons x1 tl1 =>
       if i = 0#u32
-      then Result.ret (x0, x1)
+      then
+        let back_'a :=
+          fun ret =>
+            let (t, t1) := ret
+            Result.ret (List.Cons t tl0, List.Cons t1 tl1)
+        Result.ret ((x0, x1), back_'a)
       else
         do
-          let i0 ← i - 1#u32
-          list_nth_mut_loop_pair_merge_loop T tl0 tl1 i0
+        let i1 ← i - 1#u32
+        let (p, back_'a) ← list_nth_mut_loop_pair_merge_loop T tl0 tl1 i1
+        let back_'a1 :=
+          fun ret =>
+            do
+            let (tl01, tl11) ← back_'a ret
+            Result.ret (List.Cons x0 tl01, List.Cons x1 tl11)
+        Result.ret (p, back_'a1)
     | List.Nil => Result.fail .panic
   | List.Nil => Result.fail .panic
 
-/- [loops::list_nth_mut_loop_pair_merge]: forward function
+/- [loops::list_nth_mut_loop_pair_merge]:
    Source: 'src/loops.rs', lines 223:0-227:27 -/
 def list_nth_mut_loop_pair_merge
-  (T : Type) (ls0 : List T) (ls1 : List T) (i : U32) : Result (T × T) :=
-  list_nth_mut_loop_pair_merge_loop T ls0 ls1 i
-
-/- [loops::list_nth_mut_loop_pair_merge]: loop 0: backward function 0
-   Source: 'src/loops.rs', lines 223:0-238:1 -/
-divergent def list_nth_mut_loop_pair_merge_loop_back
-  (T : Type) (ls0 : List T) (ls1 : List T) (i : U32) (ret : (T × T)) :
-  Result ((List T) × (List T))
+  (T : Type) (ls0 : List T) (ls1 : List T) (i : U32) :
+  Result ((T × T) × ((T × T) → Result ((List T) × (List T))))
   :=
-  match ls0 with
-  | List.Cons x0 tl0 =>
-    match ls1 with
-    | List.Cons x1 tl1 =>
-      if i = 0#u32
-      then let (t, t0) := ret
-           Result.ret (List.Cons t tl0, List.Cons t0 tl1)
-      else
-        do
-          let i0 ← i - 1#u32
-          let (tl00, tl10) ←
-            list_nth_mut_loop_pair_merge_loop_back T tl0 tl1 i0 ret
-          Result.ret (List.Cons x0 tl00, List.Cons x1 tl10)
-    | List.Nil => Result.fail .panic
-  | List.Nil => Result.fail .panic
+  do
+  let (p, back_'a) ← list_nth_mut_loop_pair_merge_loop T ls0 ls1 i
+  let back_'a1 := fun ret => back_'a ret
+  Result.ret (p, back_'a1)
 
-/- [loops::list_nth_mut_loop_pair_merge]: backward function 0
-   Source: 'src/loops.rs', lines 223:0-227:27 -/
-def list_nth_mut_loop_pair_merge_back
-  (T : Type) (ls0 : List T) (ls1 : List T) (i : U32) (ret : (T × T)) :
-  Result ((List T) × (List T))
-  :=
-  list_nth_mut_loop_pair_merge_loop_back T ls0 ls1 i ret
-
-/- [loops::list_nth_shared_loop_pair_merge]: loop 0: forward function
+/- [loops::list_nth_shared_loop_pair_merge]: loop 0:
    Source: 'src/loops.rs', lines 241:0-256:1 -/
 divergent def list_nth_shared_loop_pair_merge_loop
   (T : Type) (ls0 : List T) (ls1 : List T) (i : U32) : Result (T × T) :=
@@ -466,221 +387,165 @@ divergent def list_nth_shared_loop_pair_merge_loop
       then Result.ret (x0, x1)
       else
         do
-          let i0 ← i - 1#u32
-          list_nth_shared_loop_pair_merge_loop T tl0 tl1 i0
+        let i1 ← i - 1#u32
+        list_nth_shared_loop_pair_merge_loop T tl0 tl1 i1
     | List.Nil => Result.fail .panic
   | List.Nil => Result.fail .panic
 
-/- [loops::list_nth_shared_loop_pair_merge]: forward function
+/- [loops::list_nth_shared_loop_pair_merge]:
    Source: 'src/loops.rs', lines 241:0-245:19 -/
 def list_nth_shared_loop_pair_merge
   (T : Type) (ls0 : List T) (ls1 : List T) (i : U32) : Result (T × T) :=
   list_nth_shared_loop_pair_merge_loop T ls0 ls1 i
 
-/- [loops::list_nth_mut_shared_loop_pair]: loop 0: forward function
+/- [loops::list_nth_mut_shared_loop_pair]: loop 0:
    Source: 'src/loops.rs', lines 259:0-274:1 -/
 divergent def list_nth_mut_shared_loop_pair_loop
-  (T : Type) (ls0 : List T) (ls1 : List T) (i : U32) : Result (T × T) :=
+  (T : Type) (ls0 : List T) (ls1 : List T) (i : U32) :
+  Result ((T × T) × (T → Result (List T)))
+  :=
   match ls0 with
   | List.Cons x0 tl0 =>
     match ls1 with
     | List.Cons x1 tl1 =>
       if i = 0#u32
-      then Result.ret (x0, x1)
+      then
+        let back_'a := fun ret => Result.ret (List.Cons ret tl0)
+        Result.ret ((x0, x1), back_'a)
       else
         do
-          let i0 ← i - 1#u32
-          list_nth_mut_shared_loop_pair_loop T tl0 tl1 i0
+        let i1 ← i - 1#u32
+        let (p, back_'a) ← list_nth_mut_shared_loop_pair_loop T tl0 tl1 i1
+        let back_'a1 :=
+          fun ret => do
+                     let tl01 ← back_'a ret
+                     Result.ret (List.Cons x0 tl01)
+        Result.ret (p, back_'a1)
     | List.Nil => Result.fail .panic
   | List.Nil => Result.fail .panic
 
-/- [loops::list_nth_mut_shared_loop_pair]: forward function
+/- [loops::list_nth_mut_shared_loop_pair]:
    Source: 'src/loops.rs', lines 259:0-263:23 -/
 def list_nth_mut_shared_loop_pair
-  (T : Type) (ls0 : List T) (ls1 : List T) (i : U32) : Result (T × T) :=
-  list_nth_mut_shared_loop_pair_loop T ls0 ls1 i
-
-/- [loops::list_nth_mut_shared_loop_pair]: loop 0: backward function 0
-   Source: 'src/loops.rs', lines 259:0-274:1 -/
-divergent def list_nth_mut_shared_loop_pair_loop_back
-  (T : Type) (ls0 : List T) (ls1 : List T) (i : U32) (ret : T) :
-  Result (List T)
+  (T : Type) (ls0 : List T) (ls1 : List T) (i : U32) :
+  Result ((T × T) × (T → Result (List T)))
   :=
-  match ls0 with
-  | List.Cons x0 tl0 =>
-    match ls1 with
-    | List.Cons x1 tl1 =>
-      if i = 0#u32
-      then Result.ret (List.Cons ret tl0)
-      else
-        do
-          let i0 ← i - 1#u32
-          let tl00 ← list_nth_mut_shared_loop_pair_loop_back T tl0 tl1 i0 ret
-          Result.ret (List.Cons x0 tl00)
-    | List.Nil => Result.fail .panic
-  | List.Nil => Result.fail .panic
+  do
+  let (p, back_'a) ← list_nth_mut_shared_loop_pair_loop T ls0 ls1 i
+  let back_'a1 := fun ret => back_'a ret
+  Result.ret (p, back_'a1)
 
-/- [loops::list_nth_mut_shared_loop_pair]: backward function 0
-   Source: 'src/loops.rs', lines 259:0-263:23 -/
-def list_nth_mut_shared_loop_pair_back
-  (T : Type) (ls0 : List T) (ls1 : List T) (i : U32) (ret : T) :
-  Result (List T)
-  :=
-  list_nth_mut_shared_loop_pair_loop_back T ls0 ls1 i ret
-
-/- [loops::list_nth_mut_shared_loop_pair_merge]: loop 0: forward function
+/- [loops::list_nth_mut_shared_loop_pair_merge]: loop 0:
    Source: 'src/loops.rs', lines 278:0-293:1 -/
 divergent def list_nth_mut_shared_loop_pair_merge_loop
-  (T : Type) (ls0 : List T) (ls1 : List T) (i : U32) : Result (T × T) :=
+  (T : Type) (ls0 : List T) (ls1 : List T) (i : U32) :
+  Result ((T × T) × (T → Result (List T)))
+  :=
   match ls0 with
   | List.Cons x0 tl0 =>
     match ls1 with
     | List.Cons x1 tl1 =>
       if i = 0#u32
-      then Result.ret (x0, x1)
+      then
+        let back_'a := fun ret => Result.ret (List.Cons ret tl0)
+        Result.ret ((x0, x1), back_'a)
       else
         do
-          let i0 ← i - 1#u32
-          list_nth_mut_shared_loop_pair_merge_loop T tl0 tl1 i0
+        let i1 ← i - 1#u32
+        let (p, back_'a) ←
+          list_nth_mut_shared_loop_pair_merge_loop T tl0 tl1 i1
+        let back_'a1 :=
+          fun ret => do
+                     let tl01 ← back_'a ret
+                     Result.ret (List.Cons x0 tl01)
+        Result.ret (p, back_'a1)
     | List.Nil => Result.fail .panic
   | List.Nil => Result.fail .panic
 
-/- [loops::list_nth_mut_shared_loop_pair_merge]: forward function
+/- [loops::list_nth_mut_shared_loop_pair_merge]:
    Source: 'src/loops.rs', lines 278:0-282:23 -/
 def list_nth_mut_shared_loop_pair_merge
-  (T : Type) (ls0 : List T) (ls1 : List T) (i : U32) : Result (T × T) :=
-  list_nth_mut_shared_loop_pair_merge_loop T ls0 ls1 i
-
-/- [loops::list_nth_mut_shared_loop_pair_merge]: loop 0: backward function 0
-   Source: 'src/loops.rs', lines 278:0-293:1 -/
-divergent def list_nth_mut_shared_loop_pair_merge_loop_back
-  (T : Type) (ls0 : List T) (ls1 : List T) (i : U32) (ret : T) :
-  Result (List T)
+  (T : Type) (ls0 : List T) (ls1 : List T) (i : U32) :
+  Result ((T × T) × (T → Result (List T)))
   :=
-  match ls0 with
-  | List.Cons x0 tl0 =>
-    match ls1 with
-    | List.Cons x1 tl1 =>
-      if i = 0#u32
-      then Result.ret (List.Cons ret tl0)
-      else
-        do
-          let i0 ← i - 1#u32
-          let tl00 ←
-            list_nth_mut_shared_loop_pair_merge_loop_back T tl0 tl1 i0 ret
-          Result.ret (List.Cons x0 tl00)
-    | List.Nil => Result.fail .panic
-  | List.Nil => Result.fail .panic
+  do
+  let (p, back_'a) ← list_nth_mut_shared_loop_pair_merge_loop T ls0 ls1 i
+  let back_'a1 := fun ret => back_'a ret
+  Result.ret (p, back_'a1)
 
-/- [loops::list_nth_mut_shared_loop_pair_merge]: backward function 0
-   Source: 'src/loops.rs', lines 278:0-282:23 -/
-def list_nth_mut_shared_loop_pair_merge_back
-  (T : Type) (ls0 : List T) (ls1 : List T) (i : U32) (ret : T) :
-  Result (List T)
-  :=
-  list_nth_mut_shared_loop_pair_merge_loop_back T ls0 ls1 i ret
-
-/- [loops::list_nth_shared_mut_loop_pair]: loop 0: forward function
+/- [loops::list_nth_shared_mut_loop_pair]: loop 0:
    Source: 'src/loops.rs', lines 297:0-312:1 -/
 divergent def list_nth_shared_mut_loop_pair_loop
-  (T : Type) (ls0 : List T) (ls1 : List T) (i : U32) : Result (T × T) :=
+  (T : Type) (ls0 : List T) (ls1 : List T) (i : U32) :
+  Result ((T × T) × (T → Result (List T)))
+  :=
   match ls0 with
   | List.Cons x0 tl0 =>
     match ls1 with
     | List.Cons x1 tl1 =>
       if i = 0#u32
-      then Result.ret (x0, x1)
+      then
+        let back_'b := fun ret => Result.ret (List.Cons ret tl1)
+        Result.ret ((x0, x1), back_'b)
       else
         do
-          let i0 ← i - 1#u32
-          list_nth_shared_mut_loop_pair_loop T tl0 tl1 i0
+        let i1 ← i - 1#u32
+        let (p, back_'b) ← list_nth_shared_mut_loop_pair_loop T tl0 tl1 i1
+        let back_'b1 :=
+          fun ret => do
+                     let tl11 ← back_'b ret
+                     Result.ret (List.Cons x1 tl11)
+        Result.ret (p, back_'b1)
     | List.Nil => Result.fail .panic
   | List.Nil => Result.fail .panic
 
-/- [loops::list_nth_shared_mut_loop_pair]: forward function
+/- [loops::list_nth_shared_mut_loop_pair]:
    Source: 'src/loops.rs', lines 297:0-301:23 -/
 def list_nth_shared_mut_loop_pair
-  (T : Type) (ls0 : List T) (ls1 : List T) (i : U32) : Result (T × T) :=
-  list_nth_shared_mut_loop_pair_loop T ls0 ls1 i
-
-/- [loops::list_nth_shared_mut_loop_pair]: loop 0: backward function 1
-   Source: 'src/loops.rs', lines 297:0-312:1 -/
-divergent def list_nth_shared_mut_loop_pair_loop_back
-  (T : Type) (ls0 : List T) (ls1 : List T) (i : U32) (ret : T) :
-  Result (List T)
+  (T : Type) (ls0 : List T) (ls1 : List T) (i : U32) :
+  Result ((T × T) × (T → Result (List T)))
   :=
-  match ls0 with
-  | List.Cons x0 tl0 =>
-    match ls1 with
-    | List.Cons x1 tl1 =>
-      if i = 0#u32
-      then Result.ret (List.Cons ret tl1)
-      else
-        do
-          let i0 ← i - 1#u32
-          let tl10 ← list_nth_shared_mut_loop_pair_loop_back T tl0 tl1 i0 ret
-          Result.ret (List.Cons x1 tl10)
-    | List.Nil => Result.fail .panic
-  | List.Nil => Result.fail .panic
+  do
+  let (p, back_'b) ← list_nth_shared_mut_loop_pair_loop T ls0 ls1 i
+  let back_'b1 := fun ret => back_'b ret
+  Result.ret (p, back_'b1)
 
-/- [loops::list_nth_shared_mut_loop_pair]: backward function 1
-   Source: 'src/loops.rs', lines 297:0-301:23 -/
-def list_nth_shared_mut_loop_pair_back
-  (T : Type) (ls0 : List T) (ls1 : List T) (i : U32) (ret : T) :
-  Result (List T)
-  :=
-  list_nth_shared_mut_loop_pair_loop_back T ls0 ls1 i ret
-
-/- [loops::list_nth_shared_mut_loop_pair_merge]: loop 0: forward function
+/- [loops::list_nth_shared_mut_loop_pair_merge]: loop 0:
    Source: 'src/loops.rs', lines 316:0-331:1 -/
 divergent def list_nth_shared_mut_loop_pair_merge_loop
-  (T : Type) (ls0 : List T) (ls1 : List T) (i : U32) : Result (T × T) :=
+  (T : Type) (ls0 : List T) (ls1 : List T) (i : U32) :
+  Result ((T × T) × (T → Result (List T)))
+  :=
   match ls0 with
   | List.Cons x0 tl0 =>
     match ls1 with
     | List.Cons x1 tl1 =>
       if i = 0#u32
-      then Result.ret (x0, x1)
+      then
+        let back_'a := fun ret => Result.ret (List.Cons ret tl1)
+        Result.ret ((x0, x1), back_'a)
       else
         do
-          let i0 ← i - 1#u32
-          list_nth_shared_mut_loop_pair_merge_loop T tl0 tl1 i0
+        let i1 ← i - 1#u32
+        let (p, back_'a) ←
+          list_nth_shared_mut_loop_pair_merge_loop T tl0 tl1 i1
+        let back_'a1 :=
+          fun ret => do
+                     let tl11 ← back_'a ret
+                     Result.ret (List.Cons x1 tl11)
+        Result.ret (p, back_'a1)
     | List.Nil => Result.fail .panic
   | List.Nil => Result.fail .panic
 
-/- [loops::list_nth_shared_mut_loop_pair_merge]: forward function
+/- [loops::list_nth_shared_mut_loop_pair_merge]:
    Source: 'src/loops.rs', lines 316:0-320:23 -/
 def list_nth_shared_mut_loop_pair_merge
-  (T : Type) (ls0 : List T) (ls1 : List T) (i : U32) : Result (T × T) :=
-  list_nth_shared_mut_loop_pair_merge_loop T ls0 ls1 i
-
-/- [loops::list_nth_shared_mut_loop_pair_merge]: loop 0: backward function 0
-   Source: 'src/loops.rs', lines 316:0-331:1 -/
-divergent def list_nth_shared_mut_loop_pair_merge_loop_back
-  (T : Type) (ls0 : List T) (ls1 : List T) (i : U32) (ret : T) :
-  Result (List T)
+  (T : Type) (ls0 : List T) (ls1 : List T) (i : U32) :
+  Result ((T × T) × (T → Result (List T)))
   :=
-  match ls0 with
-  | List.Cons x0 tl0 =>
-    match ls1 with
-    | List.Cons x1 tl1 =>
-      if i = 0#u32
-      then Result.ret (List.Cons ret tl1)
-      else
-        do
-          let i0 ← i - 1#u32
-          let tl10 ←
-            list_nth_shared_mut_loop_pair_merge_loop_back T tl0 tl1 i0 ret
-          Result.ret (List.Cons x1 tl10)
-    | List.Nil => Result.fail .panic
-  | List.Nil => Result.fail .panic
-
-/- [loops::list_nth_shared_mut_loop_pair_merge]: backward function 0
-   Source: 'src/loops.rs', lines 316:0-320:23 -/
-def list_nth_shared_mut_loop_pair_merge_back
-  (T : Type) (ls0 : List T) (ls1 : List T) (i : U32) (ret : T) :
-  Result (List T)
-  :=
-  list_nth_shared_mut_loop_pair_merge_loop_back T ls0 ls1 i ret
+  do
+  let (p, back_'a) ← list_nth_shared_mut_loop_pair_merge_loop T ls0 ls1 i
+  let back_'a1 := fun ret => back_'a ret
+  Result.ret (p, back_'a1)
 
 end loops
