tests/coq/hashmap_on_disk/HashmapMain_FunsExternal_Template.v
@@ -11,13 +11,13 @@ Require Import HashmapMain_Types.
 Include HashmapMain_Types.
 Module HashmapMain_FunsExternal_Template.
 
-(** [hashmap_main::hashmap_utils::deserialize]: forward function
+(** [hashmap_main::hashmap_utils::deserialize]:
     Source: 'src/hashmap_utils.rs', lines 10:0-10:43 *)
 Axiom hashmap_utils_deserialize
   : state -> result (state * (hashmap_HashMap_t u64))
 .
 
-(** [hashmap_main::hashmap_utils::serialize]: forward function
+(** [hashmap_main::hashmap_utils::serialize]:
     Source: 'src/hashmap_utils.rs', lines 5:0-5:42 *)
 Axiom hashmap_utils_serialize
   : hashmap_HashMap_t u64 -> state -> result (state * unit)
