tests/fstar-split/misc/Loops.Clauses.fst
@@ -1,0 +1,107 @@
+(** [loops]: templates for the decreases clauses *)
+module Loops.Clauses
+open Primitives
+open Loops.Types
+
+#set-options "--z3rlimit 50 --fuel 1 --ifuel 1"
+
+(** [loops::sum]: decreases clause *)
+unfold let sum_loop_decreases (max : u32) (i : u32) (s : u32) : nat =
+  if i <= max then max - i else 0
+
+(** [loops::sum_with_mut_borrows]: decreases clause *)
+unfold
+let sum_with_mut_borrows_loop_decreases (max : u32) (mi : u32) (ms : u32) : nat =
+  if max >= mi then max - mi else 0
+
+(** [loops::sum_with_shared_borrows]: decreases clause *)
+unfold
+let sum_with_shared_borrows_loop_decreases (max : u32) (i : u32) (s : u32) : nat =
+  if max >= i then max - i else 0
+
+(** [loops::clear]: decreases clause *)
+unfold let clear_loop_decreases (v : alloc_vec_Vec u32) (i : usize) : nat =
+  if i <= List.Tot.length v then List.Tot.length v - i else 0
+
+(** [loops::list_mem]: decreases clause *)
+unfold let list_mem_loop_decreases (i : u32) (ls : list_t u32) : list_t u32 =
+  ls
+
+(** [loops::list_nth_mut_loop]: decreases clause *)
+unfold
+let list_nth_mut_loop_loop_decreases (t : Type0) (ls : list_t t) (i : u32) : nat =
+  i
+
+(** [loops::list_nth_shared_loop]: decreases clause *)
+unfold
+let list_nth_shared_loop_loop_decreases (t : Type0) (ls : list_t t) (i : u32) : list_t t =
+  ls
+
+(** [loops::get_elem_mut]: decreases clause *)
+unfold
+let get_elem_mut_loop_decreases (x : usize) (ls : list_t usize) : list_t usize = ls
+
+(** [loops::get_elem_shared]: decreases clause *)
+unfold
+let get_elem_shared_loop_decreases (x : usize) (ls : list_t usize) : list_t usize =
+  ls
+
+(** [loops::list_nth_mut_loop_with_id]: decreases clause *)
+unfold
+let list_nth_mut_loop_with_id_loop_decreases (t : Type0) (i : u32) (ls : list_t t) :
+  list_t t =
+  ls
+
+(** [loops::list_nth_shared_loop_with_id]: decreases clause *)
+unfold
+let list_nth_shared_loop_with_id_loop_decreases (t : Type0) (i : u32)
+  (ls : list_t t) : list_t t =
+  ls
+
+(** [loops::list_nth_mut_loop_pair]: decreases clause *)
+unfold
+let list_nth_mut_loop_pair_loop_decreases (t : Type0) (l : list_t t) (l0 : list_t t)
+  (i : u32) : nat =
+  i
+
+(** [loops::list_nth_shared_loop_pair]: decreases clause *)
+unfold
+let list_nth_shared_loop_pair_loop_decreases (t : Type0) (l : list_t t)
+  (l0 : list_t t) (i : u32) : list_t t =
+  l
+
+(** [loops::list_nth_mut_loop_pair_merge]: decreases clause *)
+unfold
+let list_nth_mut_loop_pair_merge_loop_decreases (t : Type0) (l : list_t t)
+  (l0 : list_t t) (i : u32) : nat =
+  i
+
+(** [loops::list_nth_shared_loop_pair_merge]: decreases clause *)
+unfold
+let list_nth_shared_loop_pair_merge_loop_decreases (t : Type0) (l : list_t t)
+  (l0 : list_t t) (i : u32) : list_t t =
+  l
+
+(** [loops::list_nth_mut_shared_loop_pair]: decreases clause *)
+unfold
+let list_nth_mut_shared_loop_pair_loop_decreases (t : Type0) (l : list_t t)
+  (l0 : list_t t) (i : u32) : list_t t =
+  l
+
+(** [loops::list_nth_mut_shared_loop_pair_merge]: decreases clause *)
+unfold
+let list_nth_mut_shared_loop_pair_merge_loop_decreases (t : Type0) (l : list_t t)
+  (l0 : list_t t) (i : u32) : list_t t =
+  l
+
+(** [loops::list_nth_shared_mut_loop_pair]: decreases clause *)
+unfold
+let list_nth_shared_mut_loop_pair_loop_decreases (t : Type0) (l : list_t t)
+  (l0 : list_t t) (i : u32) : list_t t =
+  l
+
+(** [loops::list_nth_shared_mut_loop_pair_merge]: decreases clause *)
+unfold
+let list_nth_shared_mut_loop_pair_merge_loop_decreases (t : Type0) (l : list_t t)
+  (l0 : list_t t) (i : u32) : list_t t =
+  l
