tests/lean/External/Funs.lean
@@ -7,92 +7,59 @@ open Primitives
 
 namespace external
 
-/- [external::swap]: forward function
+/- [external::swap]:
    Source: 'src/external.rs', lines 6:0-6:46 -/
-def swap (T : Type) (x : T) (y : T) (st : State) : Result (State × Unit) :=
-  do
-    let (st0, _) ← core.mem.swap T x y st
-    let (st1, _) ← core.mem.swap_back0 T x y st st0
-    let (st2, _) ← core.mem.swap_back1 T x y st st1
-    Result.ret (st2, ())
+def swap
+  (T : Type) (x : T) (y : T) (st : State) : Result (State × (T × T)) :=
+  core.mem.swap T x y st
 
-/- [external::swap]: backward function 0
-   Source: 'src/external.rs', lines 6:0-6:46 -/
-def swap_back
-  (T : Type) (x : T) (y : T) (st : State) (st0 : State) :
-  Result (State × (T × T))
-  :=
-  do
-    let (st1, _) ← core.mem.swap T x y st
-    let (st2, x0) ← core.mem.swap_back0 T x y st st1
-    let (_, y0) ← core.mem.swap_back1 T x y st st2
-    Result.ret (st0, (x0, y0))
-
-/- [external::test_new_non_zero_u32]: forward function
+/- [external::test_new_non_zero_u32]:
    Source: 'src/external.rs', lines 11:0-11:60 -/
 def test_new_non_zero_u32
   (x : U32) (st : State) : Result (State × core.num.nonzero.NonZeroU32) :=
   do
-    let (st0, o) ← core.num.nonzero.NonZeroU32.new x st
-    core.option.Option.unwrap core.num.nonzero.NonZeroU32 o st0
+  let (st1, o) ← core.num.nonzero.NonZeroU32.new x st
+  core.option.Option.unwrap core.num.nonzero.NonZeroU32 o st1
 
-/- [external::test_vec]: forward function
+/- [external::test_vec]:
    Source: 'src/external.rs', lines 17:0-17:17 -/
 def test_vec : Result Unit :=
   do
-    let v := alloc.vec.Vec.new U32
-    let _ ← alloc.vec.Vec.push U32 v 0#u32
-    Result.ret ()
+  let v := alloc.vec.Vec.new U32
+  let _ ← alloc.vec.Vec.push U32 v 0#u32
+  Result.ret ()
 
 /- Unit test for [external::test_vec] -/
 #assert (test_vec == Result.ret ())
 
-/- [external::custom_swap]: forward function
+/- [external::custom_swap]:
    Source: 'src/external.rs', lines 24:0-24:66 -/
 def custom_swap
-  (T : Type) (x : T) (y : T) (st : State) : Result (State × T) :=
-  do
-    let (st0, _) ← core.mem.swap T x y st
-    let (st1, x0) ← core.mem.swap_back0 T x y st st0
-    let (st2, _) ← core.mem.swap_back1 T x y st st1
-    Result.ret (st2, x0)
-
-/- [external::custom_swap]: backward function 0
-   Source: 'src/external.rs', lines 24:0-24:66 -/
-def custom_swap_back
-  (T : Type) (x : T) (y : T) (st : State) (ret : T) (st0 : State) :
-  Result (State × (T × T))
+  (T : Type) (x : T) (y : T) (st : State) :
+  Result (State × (T × (T → State → Result (State × (T × T)))))
   :=
   do
-    let (st1, _) ← core.mem.swap T x y st
-    let (st2, _) ← core.mem.swap_back0 T x y st st1
-    let (_, y0) ← core.mem.swap_back1 T x y st st2
-    Result.ret (st0, (ret, y0))
+  let (st1, (t, t1)) ← core.mem.swap T x y st
+  let back_'a := fun ret st2 => Result.ret (st2, (ret, t1))
+  Result.ret (st1, (t, back_'a))
 
-/- [external::test_custom_swap]: forward function
+/- [external::test_custom_swap]:
    Source: 'src/external.rs', lines 29:0-29:59 -/
 def test_custom_swap
-  (x : U32) (y : U32) (st : State) : Result (State × Unit) :=
+  (x : U32) (y : U32) (st : State) : Result (State × (U32 × U32)) :=
   do
-    let (st0, _) ← custom_swap U32 x y st
-    Result.ret (st0, ())
+  let (st1, (_, custom_swap_back)) ← custom_swap U32 x y st
+  let (_, (x1, y1)) ← custom_swap_back 1#u32 st1
+  Result.ret (st1, (x1, y1))
 
-/- [external::test_custom_swap]: backward function 0
-   Source: 'src/external.rs', lines 29:0-29:59 -/
-def test_custom_swap_back
-  (x : U32) (y : U32) (st : State) (st0 : State) :
-  Result (State × (U32 × U32))
-  :=
-  custom_swap_back U32 x y st 1#u32 st0
-
-/- [external::test_swap_non_zero]: forward function
+/- [external::test_swap_non_zero]:
    Source: 'src/external.rs', lines 35:0-35:44 -/
 def test_swap_non_zero (x : U32) (st : State) : Result (State × U32) :=
   do
-    let (st0, _) ← swap U32 x 0#u32 st
-    let (st1, (x0, _)) ← swap_back U32 x 0#u32 st st0
-    if x0 = 0#u32
-    then Result.fail .panic
-    else Result.ret (st1, x0)
+  let (st1, p) ← swap U32 x 0#u32 st
+  let (x1, _) := p
+  if x1 = 0#u32
+  then Result.fail .panic
+  else Result.ret (st1, x1)
 
 end external
